guarded/Inductives.v
@@ -2,67 +2,45 @@
 From MetaCoq.Checker Require Import Checker. 
 From MetaCoq.Template Require Import utils BasicAst Ast AstUtils.
 From MetaCoq.Template Require Import Universes Environment Reflect LiftSubst. 
-From MetaCoq.Template.utils Require Import RTree. 
-From MetaCoq.Template Require Import utils.Except.
+From MetaCoq.Template.utils Require Import MCRTree. 
+
+From MetaCoq.Guarded Require Import Except Trace util.
+
+(** List of known defects:
+  - The used MetaCoq reduction (from the Checker) does not handle projections.
+  - constants and constant unfolding is not handled faithfully in MetaCoq. 
+    The guardedness checker will be able to unfold constants even when they should be opaque.
+*)
 
 
+(** Exceptions *)
 
-(* TODO move *)
-Definition list_iter {X} (f : X -> exc unit) (l : list X) : exc unit := 
-  List.fold_left (fun (acc : exc unit) x => _ <- acc;; f x) l (ret tt).
-Definition list_iteri {X} (f : nat -> X -> exc unit) (l : list X) : exc unit := 
-  _ <- List.fold_left (fun (acc : exc nat) x => i <- acc;; _ <- f i x;; ret (S i)) l (ret 0);;
-  ret tt.
-(* TODO:move*)
-Definition map2_i { A B C} (f : nat -> A -> B -> C) (a : list A) (b : list B) := 
-  let map2' := fix rec a b n := 
-     match a, b with
-     | a0 :: a, b0 :: b => f n a0 b0 :: rec a b (S n)
-     | _, _ => []
-     end
-  in map2' a b 0.
-(* TODO: move *)
-Fixpoint update_list {X} (l : list X) index x := 
-  match l with 
-  | [] => []
-  | h :: l => 
-      match index with 
-      | 0 => x :: l
-      | S index => h :: update_list l index x
-      end
-  end.
-(* TODO move *)
-Definition assert (b : bool) (err : string) : exc unit := 
-  match b with 
-  | false => raise err
-  | true => ret tt
-  end.
+Notation loc := string (only parsing).
+Inductive guard_exc := 
+  | ProgrammingErr (w : loc) (s : string)
+  | OtherErr (w : loc) (s : string)
+  | EnvErr (w: loc) (kn : kername) (s : string)
+  | IndexErr (w : loc) (s : string) (i : nat)
+  | GuardErr (w : loc) (s : string)
+  | TimeoutErr. 
 
-(* TODO : move *)
-(* catch error and potentially emit another error *)
-Definition catchE {X} (a : exc X) (f : string -> exc X) : exc X := 
-  match a with 
-  | inl a => ret a
-  | inr e => f e
-  end.
+Definition max_steps := 250. 
+  
+Instance: Monad (@TraceM guard_exc) := @trace_monad max_steps guard_exc TimeoutErr. 
+Notation "'exc' A" := (@TraceM guard_exc A) (at level 100). 
+Definition unwrap := @trc_unwrap.
+Arguments unwrap { _ _ _ _}. 
 
-Definition catch {X} (a : exc X) (f : string -> X) : X := 
-  match a with 
-  | inl a => a
-  | inr e => f e
-  end.
+Instance: TrcUnwrap list := list_trc_unwrap max_steps TimeoutErr.
 
-Definition catchMap {X Y} (e : exc X) (f : string -> Y) (g : X -> Y) :=
-  match e with
-  | inr e => f e
-  | inl a => g a 
-  end.
+Notation "a == b" := (eqb a b) (at level 90). 
+Notation "a != b" := (negb(a==b)) (at level 90).
+
+(* As the guardedness checker reduces terms at many places before reducing, the key functions are not structurally recursive. 
+  We therefore disable the guardedness checker for this file. *)
+Unset Guard Checking. 
 
 
-
-(* TODO move *)
-(* head-normalized constructor types so that their conclusion exposes the inductive type -- context contains the arguments (including lets and parameters) *)
-Definition ind_ctors_hnf (i : mind_specif) := map (fun t => decompose_let_prod_env t) (ind_user_lc i).
 
 (** ** Compute uniform parameters *)
 
@@ -106,143 +84,24 @@ Definition num_uniform_params (mib : mutual_inductive_body) : nat :=
   List.fold_left (fun acc oib => min acc (one_inductive_num_uniform (mib, oib))) mib.(ind_bodies) mib.(ind_npars). 
 
 
-(* Kernel representation of lists *)
-Definition list_indname : inductive := 
-  {|
-   inductive_mind := (MPfile ["Datatypes"; "Init"; "Coq"], "list");
-   inductive_ind := 0 
-  |}.
-  
-(* NOTE: the constructor arguments in recargs trees are always without lets and without params! *)
-Definition list_recargs : wf_paths := 
-  Rec 0 [ Node (Mrec list_indname) [ Node Norec []; Node Norec [ Node Norec []; 
-                                                                 Param 0 1]
-                                   ]
-        ].
-Eval cbn in (expand (list_recargs)). 
 
-(*Inductive test := *)
-  (*| abc : let a := 10 * 10 in nat -> test. *)
-
-(*Eval hnf in let a := 10 * 10 in nat -> test.*)
-
-Print one_inductive_body.
-(* I don't really care about universes, just use Set everywhere *)
-
-Definition list_indbody : one_inductive_body := 
-  {| 
-    ind_name := "list";
-    ind_type := tProd {| binder_name := nNamed "A"; binder_relevance := Relevant |}
-                      (tSort (Universe.of_levels (inr (Level.Level "Coq.Init.Datatypes.60"))))
-                      (tSort (Universe.from_kernel_repr (Level.lSet, false) [(Level.Level "Coq.Init.Datatypes.60", false)]));
-    ind_kelim := InType;
-    ind_ctors := [("nil", tProd {|
-                               binder_name := nNamed "A";
-                               binder_relevance := Relevant |}
-                             (tSort
-                                (Universe.of_levels
-                                   (inr
-                                      (Level.Level "Coq.Init.Datatypes.60"))))
-                             (tApp (tRel 1) [tRel 0]), 0);
-                          ("cons",
-                          tProd
-                            {|
-                            binder_name := nNamed "A";
-                            binder_relevance := Relevant |}
-                            (tSort
-                               (Universe.of_levels
-                                  (inr
-                                     (Level.Level "Coq.Init.Datatypes.60"))))
-                            (tProd
-                               {|
-                               binder_name := nAnon;
-                               binder_relevance := Relevant |} 
-                               (tRel 0)
-                               (tProd
-                                  {|
-                                  binder_name := nAnon;
-                                  binder_relevance := Relevant |}
-                                  (tApp (tRel 2) [tRel 1])
-                                  (tApp (tRel 3) [tRel 2]))), 2)];
-               ind_projs := [];
-               ind_relevance := Relevant;
-               ind_recargs := list_recargs |}. 
-
-
-
-(* I don't care about universes. *)
-Definition univdecl := Monomorphic_ctx
-                   (LevelSetProp.of_list
-                      [Level.Level "Coq.Init.Datatypes.60"],
-                   ConstraintSet.empty).
-
-
-Definition list_param_ctxt := 
-[{|
-   decl_name := {|
-                binder_name := nNamed "A";
-                binder_relevance := Relevant |};
-   decl_body := None;
-   decl_type := tSort
-                  (Universe.of_levels
-                     (inr (Level.Level "Coq.Init.Datatypes.60"))) |}].
-Definition list_mindbody : mutual_inductive_body := 
-  {| 
-    ind_bodies := [list_indbody];
-    ind_finite := Finite;
-    ind_npars := 1;
-    (*ind_npars_unif := 1;*)
-    ind_params := list_param_ctxt;
-    ind_universes := univdecl;
-    ind_variance := None;
-  |}.
-
-
-Compute (num_uniform_params list_mindbody). 
-
-
-
-
-
-
-
-
-
-
-
-
-
-
-Notation "a == b" := (eqb a b) (at level 90). 
-Notation "a != b" := (negb(a==b)) (at level 90).
-
-
-
-(** * WIP : An implementation of the guardedness checker *)
-
-(* dest_subterms *)
-Definition wf_paths_constr_args_sizes t : exc (list (list wf_paths)) := 
-  destruct_node t (fun ra constrs => 
-    assert (match ra with Norec => false | _ => true end) "wf_paths_constr_args_sizes should not be called with Norec";;
-    l <- exc_unwrap $ map (fun t => destruct_node t (fun _ args => ret args) (raise "expected node")) constrs;;
-    ret l)
-  (raise "expected node").
-
-
+(** * An implementation of the guardedness checker *)
 Implicit Types (Σ : global_env) (Γ : context). 
-Definition whd_all Σ c t := 
-  except "whd_all: out of fuel" $ reduce_opt RedFlags.default Σ c default_fuel t. 
+Implicit Types (kn : kername) (c: term).
+
+(** ** Reduction and Environment Handling *)
+Definition whd_all Σ Γ t : exc term := 
+  except (OtherErr "whd_all" "out of fuel") $ reduce_opt RedFlags.default Σ Γ default_fuel t. 
 
 (* β, ι, ζ weak-head reduction *)
-Definition whd_βιζ Σ Γ t := 
+Definition whd_βιζ Σ Γ t : exc term := 
   let redflags := RedFlags.mk true true true false false false in
-  except "whd_βιζ: out of fuel" $ reduce_opt redflags Σ Γ default_fuel t. 
+  except (OtherErr "whd_βιζ" "out of fuel") $ reduce_opt redflags Σ Γ default_fuel t. 
 
 (* no let/ζ reduction *)
-Definition whd_all_nolet Σ Γ t := 
+Definition whd_all_nolet Σ Γ t : exc term := 
   let redflags := RedFlags.mk true true false true true true in
-  except "whd_all_nolet: out of fuel" $ reduce_opt redflags Σ Γ default_fuel t. 
-
+  except (OtherErr "whd_all_nolet" "out of fuel") $ reduce_opt redflags Σ Γ default_fuel t. 
 
 Definition lookup_env_const Σ kn : option constant_body := 
   match lookup_env Σ kn with 
@@ -250,8 +109,7 @@ Definition lookup_env_const Σ kn : option constant_body :=
   | _ => None
   end.
 
-
-(* TODO: what is the MetaCoq invariant here? Is the cst_body really only present when it is a transparent constant? *)
+(* NOTE: this does not accurately model the intended behaviour as MetaCoq ignores opaqueness *)
 Definition is_evaluable_const Σ kn := 
   match lookup_env_const Σ kn with
   | Some const =>
@@ -262,34 +120,35 @@ Definition is_evaluable_const Σ kn :=
   | _ => false
   end.
 
-(* TODO: same as above -- are we really allowed to reduce this?*)
+(* NOTE: same as above -- are we really allowed to reduce this?*)
 Definition get_const_value Σ kn : option term := 
   match lookup_env_const Σ kn with
   | Some const => const.(cst_body)
   | None => None
   end.
 
-Definition lookup_env_mind Σ kn : option mutual_inductive_body := 
+(* lookup a mutual inductive *)
+Definition lookup_mib Σ kn : exc mutual_inductive_body := 
   match lookup_env Σ kn with 
-  | Some (InductiveDecl ind) => Some ind
-  | _ => None
+  | Some (InductiveDecl ind) => ret ind
+  | _ => raise $ EnvErr "lookup_mib" kn "could not find inductive in global env"
   end.
 
+(* lookup an inductive *)
 Definition lookup_mind_specif Σ (ind : inductive) : exc mind_specif := 
-  mib <- except "lookup_mind_specif: could not find inductive" $ 
-    lookup_env_mind Σ ind.(inductive_mind) ;;
-  ib <- except "lookup_mind_specif: invalid inductive index" $ 
-    nth_error mib.(ind_bodies) ind.(inductive_ind) ;;
+  mib <- lookup_mib Σ ind.(inductive_mind) ;;
+  ib <- except (IndexErr "lookup_mind_specif" "invalid inductive index" ind.(inductive_ind)) $ 
+    nth_error mib.(ind_bodies) ind.(inductive_ind);;
   ret (mib, ib).
 
 
-(* if c evaluates to an application (weak-head) and the LHS is an inductive, return it together with the RHS (list) *)
-Definition find_rectype Σ Γ t := 
+(* if [t] evaluates to an application (weak-head) and the LHS is an inductive, return it together with the RHS (list) *)
+Definition find_rectype Σ Γ t : exc inductive * Instance.t * list term:= 
   t <- whd_all Σ Γ t;; 
   let (t, l) := decompose_app t in 
   match t with 
   | tInd i u => ret ((i, u), l)
-  | _ => raise "find_rectype"
+  | _ => raise $ OtherErr "find_rectype" "head is not an inductive"
   end. 
 
 
@@ -297,25 +156,21 @@ Definition find_rectype Σ Γ t :=
 Definition find_inductive Σ Γ t := 
   '((i, u), l) <- find_rectype Σ Γ t;;
   '(mib, _) <- lookup_mind_specif Σ i;;
-  if mib.(ind_finite) != CoFinite then ret ((i, u), l) else raise "find_inductive: is cofinite".
+  if mib.(ind_finite) != CoFinite then ret ((i, u), l) 
+    else raise $ OtherErr "find_inductive" "inductive is cofinite".
 
 (* only if coinductive *)
 Definition find_coinductive Σ Γ t := 
   '((i, u), l) <- find_rectype Σ Γ t;;
   '(mib, _) <- lookup_mind_specif Σ i;;
-  if mib.(ind_finite) == CoFinite then ret ((i, u), l) else raise "find_coinductive: is not cofinite".
-
+  if mib.(ind_finite) == CoFinite then ret ((i, u), l) 
+    else raise $ OtherErr "find_coinductive" "inductive is not cofinite".
 
 (* push assumptions to the de Bruijn context *)
 Definition push_assumptions_context '(names, types) Γ := 
   (* we use fold_left, so the i-th element that is pushed to the context needs to be lifted by i *)
   let ctxt := map2_i (fun i name type => vass name (lift0 i type)) names types in
   List.fold_left (fun acc assum => acc ,, assum) Γ ctxt. 
-
-
-Definition mfix_names (fixp : mfixpoint term) := map dname fixp. 
-Definition mfix_types (fixp : mfixpoint term) := map dtype fixp.
-Definition mfix_bodies (fixp : mfixpoint term) := map dbody fixp.
 
 (* [decompose_lam_assum Σ Γ ty] decomposes [ty] into a context of lambdas/lets and a remaining type, after reducing *)
 Unset Guard Checking.
@@ -363,8 +218,6 @@ Definition decompose_prod Σ Γ (t : term) : exc (context * term) :=
     end
   in decrec Γ [] t. 
 
-(* TODO: check order of arguments of vdef everywhere *)
-
 (* [decompose_lam_n_assum Σ Γ n t] decomposes [t] into a context of lambdas and lets. 
   We expect [n] lambdas and also take all the lets up to the n-th lambda, but no more lets after the n-th lambda. *)
 Definition decompose_lam_n_assum Σ Γ n (t : term) : exc (context * term) := 
@@ -379,502 +232,29 @@ Definition decompose_lam_n_assum Σ Γ n (t : term) : exc (context * term) :=
                 let d := vdef x def ty in 
                 lamdec_rec (Γ ,, d) (Γ0 ,, d) (S n) body
              | tCast t _ _ => lamdec_rec Γ Γ0 (S n) t
-             | _ => raise "decompose_lam_n_assum: not enough abstractions"
+             | _ => raise $ OtherErr "decompose_lam_n_assum" "not enough abstractions"
              end
     end
   in lamdec_rec Γ [] n t. 
 
 
-(** * Guard condition *)
-
-
-(** Environments annotated with marks on recursive arguments *)
-
-(* proper subterm (strict) or loose subterm (may be equal to the recursive argument, i.e. no proper subterm) *)
-Inductive size := Loose | Strict. 
-(* induces a lattice with Loose < Strict *)
-
-Definition size_eqb (s1 s2 : size) := 
-  match s1, s2 with 
-  | Loose, Loose => true
-  | Strict, Strict => true
-  | _, _ => false
-  end.
-Instance reflect_size : ReflectEq size.
-Proof. 
-  refine {| eqb := size_eqb |}. 
-  intros [] []; constructor; congruence. 
-Defined.
-
-(* greatest lower bound/infimum *)
-Definition size_glb s1 s2 := 
-  match s1, s2 with 
-  | Strict, Strict => Strict
-  | _, _ => Loose
-  end.
-
-(* possible specifications for a term:
-   - Not_subterm: when the size of a term is not related to the
-     recursive argument of the fixpoint
-   - Subterm: when the term is a subterm of the recursive argument
-     the wf_paths argument specifies which subterms of the term are recursive -- this is just the whole recursive structure of the term's type again, for nested matches (possibly not the trivial recargs tree that could also be looked up in the environment, but for nested inductives, this is instantiated)
-   - Dead_code: when the term has been built by elimination over an empty type
- *) 
-
-Inductive subterm_spec := 
-  | Subterm (s : size) (r : wf_paths)
-  | Dead_code
-  | Not_subterm. 
-
-Definition subterm_spec_eqb (s1 s2 : subterm_spec) := 
-  match s1, s2 with
-  | Dead_code, Dead_code => true
-  | Not_subterm, Not_subterm => true
-  | Subterm size1 tree1, Subterm size2 tree2 => 
-      (size1 == size2) && (tree1 == tree2)
-  | _, _ => false
-  end.
-Instance reflect_subterm_spec : ReflectEq subterm_spec.
-Proof. 
-  refine {| eqb := subterm_spec_eqb |}.  
-  intros [] []; unfold subterm_spec_eqb; finish_reflect. 
-Defined. 
-
-(* in contrast to the Boolean equality decider we get by eqb, this also checks equivalence if structural equality is failing *)
-Definition eq_wf_paths : wf_paths -> wf_paths -> bool := rtree_equal (eqb (A := recarg)). 
-
-(* TODO: where exactly do we need intersections *)
-Definition inter_recarg r1 r2 := 
-  match r1, r2 with
-  | Norec, Norec => Some Norec
-  | Mrec i1, Mrec i2
-  | Imbr i1, Imbr i2
-  | Mrec i1, Imbr i2 => if i1 == i2 then Some r1 else None (* intersection is an Mrec, not an Imbr, if one is an Mrec *)
-  | Imbr i1, Mrec i2 => if i1 == i2 then Some r2 else None
-  | _, _ => None
-  end.
-
-Definition inter_wf_paths := rtree_inter (eqb (A := recarg)) inter_recarg Norec. 
-Definition incl_wf_paths := rtree_incl (eqb (A := recarg)) inter_recarg Norec. 
-Definition equal_wf_paths := rtree_equal (eqb (A := recarg)). 
-
-
-Definition mk_norec := mk_node Norec []. 
-
-(* Given a list of lists with the trees for the arguments (excluding parameters) of each constructor, 
-  construct the tree for a particular inductive type. 
-  (This is not really a fully correct tree, as this is just the tree for one of the mutual inductives.) *)
-Definition mk_ind_paths rarg constr_arg_trees : wf_paths := 
-  mk_node rarg (map (fun c => mk_node Norec c) constr_arg_trees). 
-
-(* given a tree specifying the recursive structure of a term, generate a subterm spec *)
-(* used e.g. when destructing an inductive *)
-Definition spec_of_tree t := 
-  if eq_wf_paths t mk_norec then Not_subterm else Subterm Strict t. 
-
-
-(* intersection of subterm specs.
-  Dead_code is neutral element and Not_subterm least element. For Subterms, we intersect the recursive paths and the size *)
-Definition inter_spec s1 s2 : exc subterm_spec := 
-  match s1, s2 with 
-  | _, Dead_code => ret s1
-  | Dead_code, _ => ret s2
-  | Not_subterm, _ => ret s1
-  | _, Not_subterm => ret s2
-  | Subterm a1 t1, Subterm a2 t2 => 
-      inter <- except "inter_spec" $ inter_wf_paths t1 t2;;
-      ret $ Subterm (size_glb a1 a2) inter
-  end.
-
-(* greatest lower bound of a list of subterm specs *)
-Definition subterm_spec_glb (sl : list subterm_spec) : exc subterm_spec := 
-  List.fold_left (fun acc s => acc <- acc;; inter_spec acc s) sl (ret Dead_code). 
-
-(** Environment to keep track of guardedness information *)
-Record guard_env := 
-  { 
-    (* the local environment *)
-    loc_env : context;
-    (* de Bruijn index of the last fixpoint in this block (starting at 0) *)
-    (* i.e. in a block of n fixpoints, the dBs of the fixes are:
-        rel_min, ..., rel_min + n - 1
-    *)
-    rel_min_fix : nat;
-    (* de Bruijn context containing subterm information *)
-    guarded_env : list subterm_spec;
-  }.
-Implicit Type (G : guard_env). 
-
-(* make an initial guard_env after entering a fixpoint.
-  [recarg] is the index of the recursive argument, starting at 0. 
-    e.g. for [fix r (n1 : nat) (n2 : nat) {struct n1} := ....] it would be 0.
-  [tree] is the recursion tree for the inductive type of the recursive argument 
-*)
-Definition init_guard_env Γ recarg tree :=
-  {| 
-    loc_env := Γ;
-    (* Rel 0 -> recursive argument, 
-       Rel recarg -> first "proper" (non-recursive) argument,
-       Rel (S recarg) -> last fixpoint in this block 
-    *)
-    rel_min_fix := 1 + recarg;
-    guarded_env := [Subterm Loose tree]
-  |}.
-
-(* push a binder with name [na], type [type] and subterm specification [spec] *)
-Definition push_guard_env G '(na, type, spec) := 
-  {|
-    loc_env := G.(loc_env) ,, vass na type;
-    rel_min_fix := S (G.(rel_min_fix));
-    guarded_env := spec :: G.(guarded_env);
-  |}.
-
-(* update the subterm spec of dB [i] to [new_spec] *)
-Definition update_guard_spec G i new_spec := 
-  {| 
-    loc_env := G.(loc_env);
-    rel_min_fix := G.(rel_min_fix);
-    guarded_env := update_list G.(guarded_env) i new_spec 
-  |}.
-
-(* add a new inner variable which is not a subterm *)
-Definition push_nonrec_guard_env G '(na, type) := 
-  push_guard_env G (na, type, Not_subterm).
-
-(* lookup subterm information for de Bruijn index [p] *)
-Definition lookup_subterm G p := 
-  match nth_error G.(guarded_env) p with 
-  | Some spec => spec
-  | None => Not_subterm
-  end.
-
-(* push a local context -- these are not subterms *)
-Definition push_context_guard_env G Γ := 
-  let n := length Γ in 
-  {| 
-    loc_env := Γ ++ G.(loc_env);
-    rel_min_fix := G.(rel_min_fix) + n;
-    guarded_env := Nat.iter n (fun acc => Not_subterm :: acc) G.(guarded_env);
-  |}. 
-
-(* push fixes to the guard env -- these are not subterms *)
-Definition push_fix_guard_env G (mfix : mfixpoint term) := 
-  let n := length mfix in
-  {|
-    loc_env := push_assumptions_context (mfix_names mfix, mfix_types mfix) G.(loc_env);
-    rel_min_fix := G.(rel_min_fix) + n;
-    guarded_env := Nat.iter n (fun acc => Not_subterm :: acc) G.(guarded_env);
-  |}.
-
-
-(** ** Stack *)
-(* A stack is used to maintain subterm information for elements which are (morally) applied to the term currently under observation, and which would really be applied if we could fully reduce with concrete values. 
-  [SClosure] is used for efficiency reasons: we don't want to compute subterm information for everything, so this is done on demand. It thus captures the term and the guardedness environment it's in.
-  [SArg] represents subterm information for a term for which we actually have computed that information. *)
-Inductive stack_element := 
-  | SClosure G (t : term)
-  | SArg (s : subterm_spec). 
-
-(* push a list of closures [l] with guard env [G] to the stack *)
-Definition push_stack_closures G l stack := 
-  List.fold_right (fun h acc => (SClosure G h) :: acc) l stack. 
-
-(* push a list of args [l] to the stack *)
-Definition push_stack_args l stack := 
-  List.fold_right (fun h acc => SArg h :: acc) l stack. 
-
-
-(* TODO *)
-Definition hd {X} (l : list X) : exc X := 
-  match l with 
-  | [] => raise "cannot take hd of empty list"
-  | x :: l => ret x
-  end.
-
-Definition tl {X} (l : list X) : exc list X := 
-  match l with 
-  | [] => raise "cannot take tl of empty list"
-  | x :: l => ret l
-  end.
-
-
-Definition destruct_recarg (t : wf_paths) := destruct_node t (fun r _ => Some r) None. 
-
-Definition match_recarg_inductive (ind : inductive) (r : recarg) := 
-  match r with
-  | Norec => false
-  | Mrec i | Imbr i => i == ind
-  end.
-
-
-
-(* TODO move *)
 (* pseudo-reduction rule:
- * [hnf_prod_app env (Prod(_,B)) r --> B[r]
- * with an HNF on the first argument to produce a product. *)
+ * [hnf_prod_app env (Prod(_,B)) r] --> [B[r]]
+ * with a HNF on [t] to produce a product. *)
 Definition hnf_prod_app Σ Γ t r : exc term := 
   t_whd <- whd_all Σ Γ t;;
   match t_whd with 
   | tProd _ _ body => ret $ subst10 r t
-  | _ => raise "hnf_prod_app: need a product"
+  | _ => raise $ OtherErr "hnf_prod_app" "need a product"
   end.
+(* use the previous reduction to apply a list of arguments [l] to [t]. *)
 Definition hnf_prod_apps Σ Γ t l : exc term := 
   List.fold_left (fun acc r => acc <- acc;; hnf_prod_app Σ Γ acc r) l (ret t). 
 
 
-(* Add the types of mutual inductives as assumptions to the local context. 
-  The inductive types are instantiated with the (uniform) parameters in [pars]. 
-*)
-Definition context_push_ind_with_params Σ Γ (mib : mutual_inductive_body) (pars : list term) : exc context := 
-  let num_bodies := length mib.(ind_bodies) in
-  (* get relevance *)
-  fst_body <- except "mutual inductive has no bodies" $ nth_error mib.(ind_bodies) 0;;
-  let relev := fst_body.(ind_relevance) in
-  (* function: push one inductive to the context *)
-  let push_ind := fun (specif : one_inductive_body) Γ =>
-    let na := {|binder_name := nAnon; binder_relevance := relev|} in
-    (* get the type instantiated with params *)
-    ty_inst <- hnf_prod_apps Σ Γ specif.(ind_type) pars;;
-    ret $ Γ ,, vass na ty_inst 
-  in 
-  List.fold_right (fun i acc => acc <- acc;; push_ind i acc) (ret Γ) mib.(ind_bodies).
-
-(* Add the types of mutual inductives to a recargs environment *)
-Definition ra_env_push_inner_inductives_with_params ra_env ind_kn ntypes := 
-  (* make inner inductive types (Imbr in the tree) with recursive references for the individual types *)
-  let rc := rev $ mapi (fun i t => (Imbr (mkInd ind_kn i), t)) 
-                       (mk_rec_calls (X := recarg) ntypes) in
-  (* lift the existing ra_env *)
-  let ra_env := map (fun '(r, t) => (r, rtree_lift ntypes t)) ra_env in
-  rc ++ ra_env. 
-
-(* puts lambdas accepting sorts 0.. n-1 (for some dummy sorts) in front of [t] (and lift [t] accordingly)*)
-(* we don't care about the exact universe as this is only relevant for checking guardedness -- it only needs to reduce afterwards *)
-Definition lam_implicit_lift n t := 
-  let anon := mkBindAnn nAnon Relevant in
-  let some_sort := tSort (Universe.make (Level.Level "guarded_implicit")) in 
-  let lambda_implicit t := tLambda anon some_sort t in 
-  Nat.iter n lambda_implicit (lift0 n t). 
-
-(* This removes global parameters of the inductive types in [constrs] (for
-   nested inductive types only) *)
-(* for instance: if [constrs] is the list of [list] constructors, 
- * then we get back (roughly): [∀ X, (λ X, Rel 2) X;
- *                              ∀ X (x : X) (l : (λ X, Rel 3) X), (λ X, Rel 4) X]
- * i.e. we assume that at index 0 (at the outside) there is [list] instantiated with a parameter 
- * and we ignore the parameter X for the recursive occurrences of [list] in the constructor. *)
-(* Note : in the types in [constrs], the dBs 0... ntyps-1 refer to the mutual inductives *)
-(* Now we substitute the references to these types *)
-(* effectively, this means that we just ignore the parameters and instead assume that at indices 1... ntypes, 
- * there are the inductive types already instantiated with some parameters *)
-Definition abstract_params_mind_constrs num_types num_params (constrs : list term) :=
-  (* if there are no parameters, there is no abstracting to do *)
-  if num_params == 0 then constrs
-  else 
-    (* make lambdas abstracting over the parameters *)
-    let make_abs := tabulate (fun i => lam_implicit_lift num_params (tRel i)) num_types in
-    (* substitute the recursive occurences of the inductive types by these abstractions *)
-
-    map (subst0 make_abs) constrs.
-
-(* Move the first [n] prods of [c] into the context as elements of non-recursive type. *)
-Fixpoint ra_env_decompose_prod Σ Γ (ra_env : list (recarg * wf_paths)) n (c : term) {struct c} : exc (context * list (recarg * wf_paths) * term) :=
-  match n with 
-  | 0 => ret (Γ, ra_env, c)
-  | S n => 
-    c_whd <- whd_all Σ Γ c;;
-    match c_whd with
-    | tProd na ty body =>
-      let Γ' := Γ ,, vass na ty in 
-      let ra_env' := (Norec, mk_norec) :: ra_env in
-      ra_env_decompose_prod Σ Γ' ra_env' n body
-    | _ => raise "ra_env_decompose_prod: not enough prods" 
-    end
-  end.
-
-(* This code is very
-close to check_positive in indtypes.ml, but does no positivity check and does not
-compute the number of recursive arguments. *)
-Unset Guard Checking. 
-(** Build the recargs tree for a term [t]. *)
-(* [tree] is used to decide when to traverse nested inductives. *)
-(* [ra_env] is used to keep track of the subterm information of dB variables. 
-   It need not bind all variables occurring in [t]: to unbound indices, we implicitly assign [Norec].*)
-Fixpoint build_recargs Σ Γ (ra_env : list (recarg * wf_paths)) (tree : wf_paths) (t : term) {struct t}: exc wf_paths := 
-  t_whd <- whd_all Σ Γ t;;
-  let '(x, args) := decompose_app t_whd in
-  match x with 
-  | tProd na type body => 
-      assert (args == []) "reduction is broken";;
-      let Γ' := Γ ,, vass na type in
-      let ra_env' := (Norec, mk_norec) :: ra_env in
-      build_recargs Σ Γ' ra_env' tree body
-  | tRel k => 
-      (* free variables are allowed and assigned Norec *)
-      catchE (k_ra <- except "" $ nth_error ra_env k;; ret (snd k_ra)) 
-            (fun _ => ret mk_norec)
-  | tInd ind _ => 
-    (* if the given tree for [t] allows it (i.e. has an inductive as label at the root), 
-      we traverse a nested inductive *)
-    match destruct_recarg tree with 
-    | None => raise "malformed recargs tree"
-    | Some (Imbr ind') | Some (Mrec ind') => 
-        if ind == ind' then build_recargs_nested Σ Γ ra_env tree ind args 
-                       else ret mk_norec
-    | _ => ret mk_norec 
-    end
-  | _ => ret mk_norec
-  end
-
-(* Create the recursive tree for a nested inductive [ind] applied to arguments [args]. *)
-(* In particular: starting from the tree [tree], we instantiate parameters suitably, according to [args], to handle nested inductives. *)
-(* [tree] is used to decide when to traverse nested inductives. *)
-(* [ra_env] is used to keep track of the subterm information of dB variables. 
-   It need not bind all variables occurring in [t]: to unbound indices, we implicitly assign [Norec].*)
-with build_recargs_nested Σ Γ (ra_env : list (recarg * wf_paths)) (tree : wf_paths) (ind: inductive) (args: list term) {struct args}: exc wf_paths := 
-  (* if the tree [tree] already disallows recursion, we don't need to go further *)
-  if equal_wf_paths tree mk_norec then ret tree else (
-  '(mib, oib) <- lookup_mind_specif Σ ind;;
-  (* determine number of (non-) uniform parameters *)
-  let num_unif_params := num_uniform_params mib in
-  let num_non_unif_params := mib.(ind_npars) - num_unif_params in
-  (* get the instantiations for the uniform parameters *)
-  (* Note that in Coq, all parameters after the first non-uniform parameter are treated as non-uniform -- thus we can just take a prefix of the list *)
-  let inst_unif := firstn num_unif_params args in
-  let num_mut_inds := length mib.(ind_bodies) in
-  (* extend the environment with the inductive definitions applied to the parameters *)
-  Γ' <- context_push_ind_with_params Σ Γ mib inst_unif;;
-  (* do the same for the ra environment: recarg is Imbr (for inner inductives), the trees are direct recursive references [Param 0 j] *)
-  let ra_env' := ra_env_push_inner_inductives_with_params ra_env ind.(inductive_mind) num_mut_inds in
-
-  (* lift the parameters we instantiate with by the number of types: 
-      the dB layout we setup is: 
-        [inductive types setup in the nested inductive], [the environment the parameters are assuming]
-      Since we insert the inductive types when we use the parameters to instantiate the recargs tree, 
-      we thus have to lift them by the number of nested types.
-  *)
-  let inst_unif_lifted := map (lift0 num_mut_inds) inst_unif in
-
-  (* In case of mutual inductive types, we use the recargs tree which was
-    computed statically. This is fine because nested inductive types with
-    mutually recursive containers are not supported -- meaning we need not instantiate in that case. 
-    In the case that there are no mutual inductives, we use the argument tree [tree].*)
-  trees <- (if num_mut_inds == 1 
-    then arg_sizes <- wf_paths_constr_args_sizes tree;; ret [arg_sizes]
-    else exc_unwrap $ map (fun oib => wf_paths_constr_args_sizes oib.(ind_recargs)) 
-      mib.(ind_bodies));;
-
-  (* Make the recargs tree for the [j]-th inductive in the block with body [oib].
-   * Essentially, we instantiate the corresponding recargs tree in [trees] with the parameters in [inst_unif]. *)
-  let mk_ind_recargs (j : nat) (oib : one_inductive_body) : exc wf_paths :=
-    let constrs := map (fun '((_, c), _) => c) oib.(ind_ctors) in
-    (* abstract the parameters of the recursive occurrences of the inductive type in the constructor types *)
-    (* we assume that at indices 1... auxntyp, the inductive types are instantiated with the parameters *)
-    let abstracted_constrs := abstract_params_mind_constrs num_mut_inds num_unif_params constrs in
-    (* build the trees for the constructors, instantiated with the uniform parameters [inst_unif] *) 
-    paths <- exc_unwrap $ mapi (fun k c => (* [k]-th constructor with abstracted type [c] *)
-        (* instantiate the abstracted constructor types with the parameters we are interested in. *)
-        c_inst <- hnf_prod_apps Σ Γ' c inst_unif_lifted;;
-        (* move non-uniform parameters into the context *) 
-        '(Γ', ra_env', c') <- ra_env_decompose_prod Σ Γ' ra_env' num_non_unif_params c_inst;;
-        (* first fetch the trees for this constructor  *)
-        constr_trees <- except "build_recargs_nested: no tree for inductive" $ nth_error trees j;;
-        arg_trees <- except "build_recargs_nested: no tree for constructor" $ nth_error constr_trees k;; 
-        (* build the trees for the constructor's arguments *)
-        build_recargs_constructors Σ Γ' ra_env' arg_trees c'
-      ) abstracted_constrs;;
-      (* make the tree for this nested inductive *)
-      ret $ mk_ind_paths (Imbr (mkInd ind.(inductive_mind) j)) paths
-  in
-  (* create the trees for all the bodies *)
-  ind_recargs <- exc_unwrap $ mapi mk_ind_recargs mib.(ind_bodies);;
-  (* now, given the bodies, make the mutual inductive trees *)
-  trees <- except "creating trees failed" $ mk_rec ind_recargs;;
-  (* return the tree for our particular inductive type *)
-  tree_ind <- except "created trees malformed" $ nth_error trees ind.(inductive_ind);;
-  ret tree_ind)
-  
-
-(* [build_recargs_constructors Σ Γ ra_env trees c] builds a list of each of the constructor [c]'s argument's recursive structures, instantiating nested inductives suitably.  
-  We assume that [c] excludes parameters -- these should already be contained in the environment. 
-
-  [trees] is a list of trees for the constructor's argument types, used to determine when to traverse nested inductive types.
-
-  [ra_env] is used to keep track of the subterm information of dB variables. 
-   It need not bind all variables occurring in [t]: to unbound indices, we implicitly assign [Norec].
-*)
-with build_recargs_constructors Σ Γ (ra_env : list (recarg * wf_paths)) (trees : list wf_paths) (c : term) {struct c}: exc (list wf_paths) := 
-  let recargs_constr_rec := fix recargs_constr_rec Γ (ra_env : list (recarg * wf_paths)) (trees : list wf_paths) (lrec :list wf_paths) (c : term) {struct c} : exc (list wf_paths) := 
-    c_whd <- whd_all Σ Γ c;;
-    let '(x, args) := decompose_app c_whd in
-    match x with 
-    | tProd na type body => 
-        (* the constructor has an argument of type [type] *)
-        assert (args == []) "reduction is broken";;
-        (* compute the recursive structure of [type] *)
-        first_tree <- hd trees;;
-        (*rec_tree <- raise "a";;*)
-        rec_tree <- build_recargs Σ Γ ra_env first_tree type;;
-        (* [na] of type [type] is non-recursive *)
-        let Γ' := Γ ,, vass na type in
-        let ra_env' := (Norec, mk_norec) :: ra_env in 
-        (* process the rest of the constructor type *)
-        rest_trees <- tl trees;;
-        recargs_constr_rec Γ' ra_env' rest_trees (rec_tree :: lrec) body
-    | _ => 
-        (* we have processed all the arguments of the constructor -- reverse to get a valid dB-indexed context *)
-        ret $ rev lrec  
-    end
-  in recargs_constr_rec Γ ra_env trees [] c. 
-
-
-(* [get_recargs_approx env tree ind args] builds an approximation of the recargs
-tree for [ind], knowing [args]. The argument [tree] is used to know when candidate
-nested types should be traversed, pruning the tree otherwise. *)
-Definition get_recargs_approx Σ Γ (tree : wf_paths) (ind : inductive) (args : list term) : exc wf_paths := 
-  (* starting with ra_env = [] seems safe because any unbound Rel will be assigned Norec *)
-  build_recargs_nested Σ Γ [] tree ind args. 
-
-
-(** ** Checking fixpoints *)
-
-
-(* Given a subterm spec for a term to match on, compute the subterm specs for the binders bound by a match in the individual branches. *)
-(* In [match c as z in ci y_s return P with |C_i x_s => t end]
-   [branches_specif Σ G c_spec ind] returns an array of x_s specs knowing
-   c_spec. *)
-(* [ind] is the inductive we match on. *)
-Definition branches_binders_specif Σ G (discriminant_spec : subterm_spec) (ind : inductive) : exc list (list subterm_spec) := 
-  (* get the arities of the constructors (without lets, without parameters) *)
-  constr_arities <- (
-    '(_, oib) <- lookup_mind_specif Σ ind;;
-    ret $ map snd oib.(ind_ctors));;
-  exc_unwrap $ mapi (fun i (ar : nat) => 
-    match discriminant_spec return exc (list subterm_spec)  with 
-    | Subterm _ tree => 
-        (* check if the tree refers to the same inductive as we are matching on *)
-        recarg_info <- except "malformed tree" $ destruct_recarg tree;;
-        if negb (match_recarg_inductive ind recarg_info) then
-          (* the tree talks about a different inductive than we are matching on, so all the constructor's arguments cannot be subterms  *)
-          ret $ tabulate (fun _ => Not_subterm) ar
-        else 
-          (* get trees for the arguments of the i-th constructor *)
-          constr_args_sizes <- wf_paths_constr_args_sizes tree;;
-          args_sizes <- except "" $ nth_error constr_args_sizes i;;
-          (* this should hopefully be long enough and agree with the arity of the constructor *)
-          assert (length args_sizes == ar) "number of constructor arguments don't agree";;
-          (* for each arg of the constructor: generate a strict subterm spec if they are recursive, otherwise Not_subterm. 
-            These do also contain the recursive tree for that argument to enable nested matches. *)
-          ret $ map spec_of_tree args_sizes 
-    | Dead_code => 
-        (* just propagate *)
-        ret $ tabulate (fun _ => Dead_code) ar
-    | Not_subterm => 
-        (* just propagate *)
-        ret $ tabulate (fun _ => Not_subterm) ar
-    end
-    ) constr_arities.
-
+Definition mfix_names (fixp : mfixpoint term) := map dname fixp. 
+Definition mfix_types (fixp : mfixpoint term) := map dtype fixp.
+Definition mfix_bodies (fixp : mfixpoint term) := map dbody fixp.
 
 (* [fold_term_with_binders g f n acc c] folds [f n] on the immediate
    subterms of [c] starting from [acc] and proceeding from left to
@@ -899,11 +279,11 @@ Definition fold_term_with_binders {X Y}(g : X -> X) (f : X -> Y -> term -> Y) (n
       List.fold_left (fun acc '(type, body) => f n' (f n acc type) body) types_and_bodies acc
   end.
 
+
+
 (* check if a de Bruijn index in range 
     n ... n + num -1 
   occurs in t *)
-Unset Guard Checking.
-(*FIXME: not strictly structural, just unset guard checking for now *)
 (* TODO: might not handle evars/metas/casts correctly *)
 Definition rel_range_occurs n num t := 
   let occur_rec := fix occur_rec n t {struct t}:= 
@@ -913,74 +293,546 @@ Definition rel_range_occurs n num t :=
     | _ => fold_term_with_binders S (fun n acc t => acc || occur_rec n t) n false t
     end
   in occur_rec n t.
-Set Guard Checking.
 
 
+Definition lookup_ind_subterms Σ (ind : inductive) :=
+  '(_, oib) <- lookup_mind_specif Σ ind;;
+  ret oib.(ind_recargs).
 
-Unset Guard Checking. 
-(* Extract the [inductive] that [fixp] is doing recursion over
-   (and check that the recursion is indeed over an inductive).
-  Moreover give the body of [fixp] after the recursive argument and the environment (updated from [Γ])
-  that contains the arguments up to (and including) the recursive argument (of course also the fixpoints). *)
-(* FIXME: is not structurally recursive as we reduce before checking *)
-Definition inductive_of_mutfix Σ Γ (fixp : mfixpoint term) : exc (list inductive * list (context * term)):= 
-  let number_of_fixes := length fixp in
-  assert (number_of_fixes != 0) "ill-formed fix";;
-  let ftypes := mfix_types fixp in
-  let fnames := mfix_names fixp in 
-  let fbodies := mfix_bodies fixp in
-  (* push fixpoints to environment *)
-  let Γ_fix := push_assumptions_context (fnames, ftypes) Γ in
-  let nvect := map rarg fixp in 
+(* check if a (function) type has an inductive co-domain *)
+Definition has_inductive_codomain Σ Γ t : exc bool := 
+  '(abs_context, t') <- decompose_lam_assum Σ Γ t;;
+  let Γ' := Γ ,,, abs_context in
+  '(context', t'') <- decompose_prod_assum Σ Γ t';;
+  let Γ'' :=  Γ' ,,, context' in
+  t''_whd <- whd_all Σ Γ'' t'';;
+  let '(i, _) := decompose_app t''_whd in
+  match i with 
+  | tInd _ _ => ret true
+  | _ => ret false 
+  end.
 
-  (* Check the i-th definition [fixdef] of the mutual inductive block where k is the recursive argument, 
-    making sure that no invalid recursive calls are in the types of the first [k] arguments, 
-    make sure that the recursion is over an inductive type, 
-    and return that inductive together with the body of [fixdef] after the recursive arguement
-    together with its context. *)
-  let find_ind i k fixdef : exc (inductive * (context * term)):= 
-      (* check that a rec call to the fixpoint [fixdef] does not appear in the [k] first abstractions,
-        that the recursion is over an inductive, and 
-        gives the inductive and the body + environment of [fixdef] after introducing the first [k] arguments *)
-      let check_occur := fix check_occur Γ n (def : term) {struct def}: exc (inductive * (context * term)) := 
-        (* n is the number of lambdas we're under/aka the dB from which the mutual fixes are starting:
-          n ... n + number_of_fixes - 1 *)
-        def_whd <- whd_all Σ Γ def;;
-        match def_whd with 
-        | tLambda x t body => 
-            assert (negb(rel_range_occurs n number_of_fixes t)) "bad occurrence of recursive call";;
-            let Γ' := Γ ,, (vass x t) in
-            if n == k then (* becomes true once we have entered [k] inner lambdas*)
-              (* so now the rec arg should be at dB 0 and [t] is the type we are doing recursion over *)
-              (* get the inductive type of the fixpoint, ensuring that it is an inductive *)
-              '((ind, _), _) <- catchE (find_inductive Σ Γ t) (fun _ => raise "recursion not on inductive");;
-              '(mib, _) <- lookup_mind_specif Σ ind;;
-              if mib.(ind_finite) != Finite then (* ensure that it is an inductive *)
-                raise "recursion not on inductive"
-              else
-                (* now return the inductive, the env after taking the inductive argument and all arguments before it, and the rest of the fix's body *)
-                ret (ind, (Γ', body))
-            else check_occur Γ' (S n) body
-        | _ => 
-            (* not a lambda -> we do not have enough arguments and can't find the recursive one *)
-            raise "not enough abstractions in fix body" 
-        end
-      in 
-      (* check that recursive occurences are nice and extract inductive + fix body *)
-      res <- check_occur Γ_fix 0 fixdef;; 
-      let '(ind, _) := res in
-      '(_, oib) <- lookup_mind_specif Σ ind;;
-      (*if oib.(ind_relevance) == Irrelevant && *)
-      (* TODO some sprop checking for relevance *)
-      ret res
+(** ** Environments for keeping track of subterm information *)
+
+(** Environments annotated with marks on recursive arguments *)
+
+(** proper subterm (strict) or loose subterm (may be equal to the recursive argument, i.e. not a proper subterm) *)
+Inductive size := Loose | Strict. 
+(* induces a lattice with Loose < Strict *)
+
+Definition size_eqb (s1 s2 : size) := 
+  match s1, s2 with 
+  | Loose, Loose => true
+  | Strict, Strict => true
+  | _, _ => false
+  end.
+Instance reflect_size : ReflectEq size.
+Proof. 
+  refine {| eqb := size_eqb |}. 
+  intros [] []; constructor; congruence. 
+Defined.
+
+(* greatest lower bound/infimum of size information *)
+Definition size_glb s1 s2 := 
+  match s1, s2 with 
+  | Strict, Strict => Strict
+  | _, _ => Loose
+  end.
+
+(* possible specifications for a term:
+   - Not_subterm: when the size of a term is not related to the recursive argument of the fixpoint
+   - Subterm: when the term is a subterm of the recursive argument
+     the [wf_paths] argument specifies which subterms of the term are recursive 
+     -- this is just the whole recursive structure of the term's type again, for nested matches 
+        (possibly not the trivial recargs tree that could also be looked up in the environment: for nested inductives, this is instantiated)
+   - Dead_code: when the term has been built by elimination over an empty type. Is also used for evars.
+ *) 
+Inductive subterm_spec := 
+  | Subterm (s : size) (r : wf_paths)
+  | Dead_code
+  | Not_subterm. 
+
+Definition subterm_spec_eqb (s1 s2 : subterm_spec) := 
+  match s1, s2 with
+  | Dead_code, Dead_code => true
+  | Not_subterm, Not_subterm => true
+  | Subterm size1 tree1, Subterm size2 tree2 => 
+      (size1 == size2) && (tree1 == tree2)
+  | _, _ => false
+  end.
+Instance reflect_subterm_spec : ReflectEq subterm_spec.
+Proof. 
+  refine {| eqb := subterm_spec_eqb |}.  
+  intros [] []; unfold subterm_spec_eqb; finish_reflect. 
+Defined. 
+
+(* In contrast to the Boolean equality decider we get by eqb, this also checks equivalence if structural equality is failing by unfolding the recursive trees. *)
+Definition eq_wf_paths : wf_paths -> wf_paths -> bool := rtree_equal (eqb (A := recarg)). 
+
+(* Join the recarg info if compatible. *)
+Definition inter_recarg r1 r2 := 
+  match r1, r2 with
+  | Norec, Norec => Some Norec
+  | Mrec i1, Mrec i2
+  | Imbr i1, Imbr i2
+  | Mrec i1, Imbr i2 => if i1 == i2 then Some r1 else None (* intersection is an Mrec, not an Imbr, if one is an Mrec *)
+  | Imbr i1, Mrec i2 => if i1 == i2 then Some r2 else None
+  | _, _ => None
+  end.
+
+(** *** Operations on recursive arguments trees *)
+
+(* TODO: where exactly do we need intersections *)
+(* Intersection and equality test on [wf_paths]. *)
+Definition inter_wf_paths := rtree_inter (eqb (A := recarg)) inter_recarg Norec. 
+Definition incl_wf_paths := rtree_incl (eqb (A := recarg)) inter_recarg Norec. 
+Definition equal_wf_paths := rtree_equal (eqb (A := recarg)). 
+
+Definition mk_norec := mk_node Norec []. 
+
+(* Given a recargs tree [t] representing for an inductive, get a list of trees for the arguments of the constructors. *)
+Definition wf_paths_constr_args_sizes t : exc (list (list wf_paths)) := 
+  destruct_node t (fun ra constrs => 
+    assert (match ra with Norec => false | _ => true end) $ ProgrammingErr "wf_paths_constr_args_sizes" "should not be called with Norec";;
+    l <- unwrap $ map (fun t => destruct_node t (fun _ args => ret args) (raise $ ProgrammingErr "wf_paths_constr_args_sizes" "expected node")) 
+      constrs;;
+    ret l)
+  (raise $ ProgrammingErr "wf_paths_constr_args_sizes" "expected node").
+
+(* Given a list of lists with the trees for the arguments (excluding parameters) of each constructor, 
+  construct the tree for a particular inductive type. 
+  (This is not really a fully correct tree, as this is just the tree for one of the mutual inductives.) *)
+Definition mk_ind_paths rarg constr_arg_trees : wf_paths := 
+  mk_node rarg (map (fun l => mk_node Norec l) constr_arg_trees). 
+
+(* Given a tree specifying the recursive structure of a term, generate a subterm spec. *)
+(* (used e.g. when matching on an element of inductive type) *)
+Definition spec_of_tree t := if eq_wf_paths t mk_norec then Not_subterm else Subterm Strict t. 
+
+(* Intersection of subterm specs. 
+   Main use: when determining the subterm info for a match, we take the glb of the subterm infos for the branches.
+*)
+(* Dead_code is neutral element and Not_subterm least element. For Subterms, we intersect the recursive paths and the size. *)
+(* Example for the handling of Dead_code:
+    <<
+      match n as n return n <> 0 -> nat with
+      | 0 => fun H => match H with end
+      | S k => fun _ => k
+      end
+    >>
+    In the above case, the first branch would get spec [Dead_code] and the second one a [Subterm]. 
+    The full match is then a [Subterm].
+*)
+Definition subterm_spec_glb2 s1 s2 : exc subterm_spec := 
+  match s1, s2 with 
+  | _, Dead_code => ret s1
+  | Dead_code, _ => ret s2
+  | Not_subterm, _ => ret s1
+  | _, Not_subterm => ret s2
+  | Subterm a1 t1, Subterm a2 t2 => 
+      inter <- except (OtherErr "subterm_spec_glb2" "inter_wf_paths failed") $ inter_wf_paths t1 t2;;
+      ret $ Subterm (size_glb a1 a2) inter
+  end.
+
+(* Greatest lower bound of a list of subterm specs. *)
+(* Important: the neutral element is [Dead_code] -- for matches over empty types, we thus get [Dead_code]. *)
+Definition subterm_spec_glb (sl : list subterm_spec) : exc subterm_spec := 
+  List.fold_left (fun acc s => acc <- acc;; subterm_spec_glb2 acc s) sl (ret Dead_code). 
+
+(** *** Guard env *)
+
+(** Environment to keep track of guardedness information *)
+Record guard_env := 
+  { 
+    (* the local environment *)
+    loc_env : context;
+    (* de Bruijn index of the last fixpoint in this block (starting at 0) *)
+    (* i.e. in a block of [n] fixpoints, the dBs of the fixes are:
+        [rel_min_fix], ..., [rel_min_fix + n - 1]
+    *)
+    rel_min_fix : nat;
+    (* de Bruijn context containing subterm information *)
+    guarded_env : list subterm_spec;
+  }.
+Implicit Type (G : guard_env). 
+
+(* Make an initial guard_env after entering a fixpoint to check.
+  [recarg] is the index of the recursive argument, starting at 0. 
+    e.g. for [fix r (n1 : nat) (n2 : nat) {struct n1} := ....] it would be 0.
+  [tree] is the recursion tree for the inductive type of the recursive argument.
+*)
+Definition init_guard_env Γ recarg tree :=
+  {| 
+    loc_env := Γ;
+    (* Rel 0 -> recursive argument, 
+       Rel recarg -> first "proper" (non-recursive) argument,
+       Rel (S recarg) -> last fixpoint in this block 
+    *)
+    rel_min_fix := 1 + recarg;
+    guarded_env := [Subterm Loose tree]
+  |}.
+
+(* Push a binder with name [na], type [type] and subterm specification [spec] *)
+Definition push_guard_env G '(na, type, spec) := 
+  {|
+    loc_env := G.(loc_env) ,, vass na type;
+    rel_min_fix := S (G.(rel_min_fix));
+    guarded_env := spec :: G.(guarded_env);
+  |}.
+
+(* add a new inner variable which is not a subterm *)
+Definition push_nonrec_guard_env G '(na, type) := 
+  push_guard_env G (na, type, Not_subterm).
+
+(* Update the subterm spec of dB [i] to [new_spec] *)
+Definition update_guard_spec G i new_spec := 
+  {| 
+    loc_env := G.(loc_env);
+    rel_min_fix := G.(rel_min_fix);
+    guarded_env := update_list G.(guarded_env) i new_spec 
+  |}.
+
+(* lookup subterm information for de Bruijn index [p] *)
+Definition lookup_subterm G p := 
+  match nth_error G.(guarded_env) p with 
+  | Some spec => spec
+  | None => Not_subterm
+  end.
+
+(* push a local context as [Not_subterm]s *)
+Definition push_context_guard_env G Γ := 
+  let n := length Γ in 
+  {| 
+    loc_env := G.(loc_env) ,,, Γ ;
+    rel_min_fix := G.(rel_min_fix) + n;
+    guarded_env := Nat.iter n (fun acc => Not_subterm :: acc) G.(guarded_env);
+  |}. 
+
+(* push fixes to the guard env as [Not_subterm]s *)
+Definition push_fix_guard_env G (mfix : mfixpoint term) := 
+  let n := length mfix in
+  {|
+    loc_env := push_assumptions_context (mfix_names mfix, mfix_types mfix) G.(loc_env);
+    rel_min_fix := G.(rel_min_fix) + n;
+    guarded_env := Nat.iter n (fun acc => Not_subterm :: acc) G.(guarded_env);
+  |}.
+
+
+(** ** Stack *)
+(* A stack is used to maintain subterm information for elements which are (morally) applied to the term currently under observation, and which would really be applied if we could fully reduce with concrete values. 
+  [SClosure] is used for efficiency reasons: we don't want to compute subterm information for everything, so this is done on demand. It thus captures the term and the guardedness environment it's in.
+  [SArg] represents subterm information for a term for which we actually have computed that information. *)
+(* Example where this is used: 
+  << 
+    match complex_fun n with 
+    | 0 => fun t => ...
+    | S n => fun t => ...
+    end k
+  >>
+  Here, the [fun t => ...] inside the match-branches would be checked with a stack having the subterm info for [k] at the head, as that term would really be applied to the [k].  
+*)
+(* (Note however that not all subterm information is allowed to flow through matches like that, see the functions below. ) *)
+Inductive stack_element := 
+  | SClosure G (t : term)
+  | SArg (s : subterm_spec). 
+
+(* Push a list of closures [l] with guard env [G] to the stack *)
+Definition push_stack_closures G l stack := 
+  List.fold_right (fun h acc => (SClosure G h) :: acc) l stack. 
+
+(* Push a list of args [l] to the stack *)
+Definition push_stack_args l stack := 
+  List.fold_right (fun h acc => SArg h :: acc) l stack. 
+
+(* Get the recarg the root node of [t] is annotated with. *)
+Definition destruct_recarg (t : wf_paths) := destruct_node t (fun r _ => Some r) None. 
+
+(* Check that the recarg [r] is an [Mrec] or [Imbr] node with [ind]. *)
+Definition match_recarg_inductive (ind : inductive) (r : recarg) := 
+  match r with
+  | Norec => false
+  | Mrec i | Imbr i => i == ind
+  end.
+
+(* Add the types of mutual inductives as assumptions to the local context (the first inductive body at dB 0)
+  The inductive types are instantiated with the (uniform) parameters in [pars]. 
+*)
+Definition context_push_ind_with_params Σ Γ (mib : mutual_inductive_body) (pars : list term) : exc context := 
+  let num_bodies := length mib.(ind_bodies) in
+  (* get relevance *)
+  fst_body <- except (OtherErr "context_push_ind_with_params" "mutual inductive has no bodies") $
+    nth_error mib.(ind_bodies) 0;;
+  let relev := fst_body.(ind_relevance) in
+  (* function: push one inductive to the context *)
+  let push_ind := fun (specif : one_inductive_body) Γ =>
+    let na := {|binder_name := nAnon; binder_relevance := relev|} in
+    (* get the type instantiated with params *)
+    ty_inst <- hnf_prod_apps Σ Γ specif.(ind_type) pars;;
+    ret $ Γ ,, vass na ty_inst 
   in 
-  (* now iterate this on all the fixpoints of the mutually recursive block *)
-  rv <- exc_unwrap $ map2_i find_ind nvect fbodies;;
-  (* return the list of inductives as well as the fixpoint bodies in their context *)
-  ret (map fst rv : list inductive, map snd rv : list (context * term)).
+  List.fold_right (fun i acc => acc <- acc;; push_ind i acc) (ret Γ) mib.(ind_bodies).
 
-(* [restrict_spec_for_match Σ Γ spec rtf] restricts the size information in [spec] to what is 
-allowed to flow through a match with return-type function [rtf] in environment (Σ, Γ). *)
+
+(** ** Building recargs trees *)
+
+
+(* TODO: the following is not really what happens. 
+  We already have a tree with a suitable instantiation of nested inductive containers (the positivity checker uses a very similar function to compute it). 
+  The following stuff to compute a new tree is only ever used to restrict the flow of information through matches.. *)
+
+(** Nested inductives need special attention: to correctly handle matches (and subterms) on elements of a nested inductive type we are doing recursion over, the inner inductive type's parameters need to be properly instantiated with the outer inductive type. This is in particular the case for the recursive arguments tree. *)
+(** Example: rose trees
+   [Inductive rtree (X : Type) := rnode (l : list (rtree X)).]
+   When we check a fixpoint which is structural over [r : rtree X] and (after matching) [r] ≃ [rnode l], 
+    we want to be able to do recursive calls with elements of [l]. 
+   In order to obtain this subterm information when matching on [l], the recargs tree for the [list] type is instantiated with [rtree] beforehand. 
+
+                Rec 0 
+                 | 
+            Node (Mrec list_ind)
+        /                           \
+    Node Norec                   Node Norec
+                                /             \
+                            Node Norec    Param 0 0
+
+  is turned into
+
+                Rec 0 
+                 | 
+            Node (Imbr list_ind)
+        /                           \
+    Node Norec                   Node Norec
+                                /             \
+                            Param 1 0      Param 0 0
+
+  where the Param 1 1 references the node for [rtree] on the outside.
+  The full tree for [rtree] is then:
+
+              Rec 0
+                |
+        Node (Mrec rtree_ind)
+                | 
+            Node Norec
+                | 
+  [the instantiated tree for list] 
+    
+*)
+
+(** To construct the recargs tree, the code makes use of [ra_env : list (recarg * wf_paths)], a de Bruijn context containing the recursive tree and the inductive for elements of an (instantiated) inductive type, and [(Norec, mk_norec)] for elements of non-inductive type.  
+
+  Importantly, the recargs tree (of type wf_paths) may make references to other elements in the [ra_env] (via the [Param] constructor).
+*)
+
+
+(** Add the types of inner mutual inductives to a recargs environment. This is used in the context of nested inductives.
+  Specifically, for the j-th inductive in the block, we add [(Imbr $ mkInd ind_kn j, Param 0 j)], i.e. an inner inductive with a direct recursive reference to the j-th inductive in the block. 
+  The rest of the env is lifted accordingly.
+  *)
+Definition ra_env_push_inner_inductives_with_params ra_env ind_kn ntypes := 
+  (* make inner inductive types (Imbr in the tree) with recursive references for the individual types *)
+  let rc := rev $ mapi (fun i t => (Imbr (mkInd ind_kn i), t)) 
+                       (mk_rec_calls (X := recarg) ntypes) in
+  (* lift the existing ra_env *)
+  let ra_env := map (fun '(r, t) => (r, rtree_lift ntypes t)) ra_env in
+  rc ++ ra_env. 
+
+
+(** Puts lambdas accepting sorts [0].. [n-1] (for some dummy sorts) in front of [t] (and lift [t] accordingly)*)
+(** We don't care about the exact universe as this is only relevant for checking guardedness -- it only needs to reduce afterwards *)
+Definition lam_implicit_lift n t := 
+  let anon := mkBindAnn nAnon Relevant in
+  let some_sort := tSort (Universe.make (Level.Level "guarded_implicit")) in 
+  let lambda_implicit t := tLambda anon some_sort t in 
+  Nat.iter n lambda_implicit (lift0 n t). 
+
+(* This removes global parameters of the inductive types in [constrs] (for nested inductive types only). *)
+(* for instance: if [constrs] is the list of [list] constructors, 
+ * then we get back (roughly): [∀ X, (λ X, Rel 2) X;
+ *                              ∀ X (x : X) (l : (λ X, Rel 3) X), (λ X, Rel 4) X]
+ * i.e. we assume that at index 0 (at the outside) there is [list] instantiated with a parameter 
+ * and we ignore the parameter X for the recursive occurrences of [list] in the constructor. *)
+(* Note : in the types in [constrs], the dBs 0... ntyps-1 refer to the mutual inductives. *)
+(* Now we substitute the references to these types. *)
+(* Effectively, this means that we just ignore the parameters and instead assume that at indices [0]... [ntypes-1], there are the inductive types already instantiated with some parameters. *)
+Definition abstract_params_mind_constrs num_types num_params (constrs : list term) :=
+  (* if there are no parameters, there is no abstracting to do *)
+  if num_params == 0 then constrs
+  else 
+    (* make lambdas abstracting over the parameters *)
+    let make_abs := tabulate (fun i => lam_implicit_lift num_params (tRel i)) num_types in
+    (* substitute the recursive occurences of the inductive types by these abstractions *)
+
+    map (subst0 make_abs) constrs.
+
+(* Move the first [n] prods of [c] into the context as elements of non-recursive type. *)
+Fixpoint ra_env_decompose_prod Σ Γ (ra_env : list (recarg * wf_paths)) n (c : term) {struct c} : exc (context * list (recarg * wf_paths) * term) :=
+  match n with 
+  | 0 => ret (Γ, ra_env, c)
+  | S n => 
+    c_whd <- whd_all Σ Γ c;;
+    match c_whd with
+    | tProd na ty body =>
+      let Γ' := Γ ,, vass na ty in 
+      let ra_env' := (Norec, mk_norec) :: ra_env in
+      ra_env_decompose_prod Σ Γ' ra_env' n body
+    | _ => raise (OtherErr "ra_env_decompose_prod" "not enough prods") 
+    end
+  end.
+
+(* Create the recursive tree for a nested inductive [ind] applied to arguments [args]. *)
+(* In particular: starting from the tree [tree], we instantiate parameters suitably (with [args]) to handle nested inductives. *)
+(* [tree] is used to decide when to traverse nested inductives. *)
+(* [ra_env] is used to keep track of the subterm information of dB variables. 
+   It need not bind all variables occurring in [t]: to unbound indices, we implicitly assign [Norec].*)
+Fixpoint build_recargs_nested Σ Γ (ra_env : list (recarg * wf_paths)) (tree : wf_paths) (ind: inductive) (args: list term) {struct args}: exc wf_paths := 
+  (* if the tree [tree] already disallows recursion, we don't need to go further *)
+  if equal_wf_paths tree mk_norec then ret tree else (
+  '(mib, oib) <- lookup_mind_specif Σ ind;;
+  (* determine number of (non-) uniform parameters *)
+  let num_unif_params := num_uniform_params mib in
+  let num_non_unif_params := mib.(ind_npars) - num_unif_params in
+  (* get the instantiations for the uniform parameters *)
+  (* Note that in Coq, all parameters after the first non-uniform parameter are treated as non-uniform -- thus we can just take a prefix of the list *)
+  let inst_unif := firstn num_unif_params args in
+  let num_mut_inds := length mib.(ind_bodies) in
+  (* extend the environment with the inductive definitions applied to the parameters *)
+  Γ' <- context_push_ind_with_params Σ Γ mib inst_unif;;
+  (* do the same for the ra environment: 
+    for the j-th inductive, 
+    the recarg is Imbr (for the container), 
+    the trees are direct recursive references [Param 0 j] *)
+  let ra_env' := ra_env_push_inner_inductives_with_params ra_env ind.(inductive_mind) num_mut_inds in
+
+  (* lift the parameters we instantiate with by the number of types: 
+    the dB layout we setup is: 
+        [inductive types defined in the container of the nested ind], [the environment the parameters are assuming]
+    Since we insert the inductive types when we use the parameters to instantiate the recargs tree, we thus have to lift the parameters by the number of mutual types of the container.
+  *)
+  let inst_unif_lifted := map (lift0 num_mut_inds) inst_unif in
+
+  (* In case of mutual inductive types, we use the recargs tree which was
+    computed statically. This is fine because nested inductive types with
+    mutually recursive containers are not supported -- meaning we need not instantiate in that case. 
+    In the case that there are no mutual inductives, we use the argument tree [tree].*)
+  trees <- (if num_mut_inds == 1 
+    then arg_sizes <- wf_paths_constr_args_sizes tree;; ret [arg_sizes]
+    else unwrap $ map (fun oib => wf_paths_constr_args_sizes oib.(ind_recargs)) 
+      mib.(ind_bodies));;
+
+  (* function: make the recargs tree for the [j]-th inductive in the block with body [oib].
+   * Essentially, we instantiate the corresponding recargs tree in [trees] with the parameters in [inst_unif]. *)
+  let mk_ind_recargs (j : nat) (oib : one_inductive_body) : exc wf_paths :=
+    (* get constructor types (with parameters), assuming that the mutual inductives are at [0]...[num_mut_inds-1]*)
+    let constrs := map (fun '((_, c), _) => c) oib.(ind_ctors) in
+    (* abstract the parameters of the recursive occurrences of the inductive type in the constructor types *)
+    (* we assume that at indices [0]... [num_mut_inds-1], the inductive types are instantiated _with_ the parameters *)
+    let abstracted_constrs := abstract_params_mind_constrs num_mut_inds num_unif_params constrs in
+    (* build the trees for the constructors, instantiated with the uniform parameters [inst_unif] *) 
+    paths <- unwrap $ mapi (fun k c => (* [k]-th constructor with abstracted type [c] *)
+        (* instantiate the abstracted constructor types with the parameters we are interested in. *)
+        c_inst <- hnf_prod_apps Σ Γ' c inst_unif_lifted;;
+        (* move non-uniform parameters into the context *) 
+        '(Γ', ra_env', c') <- ra_env_decompose_prod Σ Γ' ra_env' num_non_unif_params c_inst;;
+        (* first fetch the trees for this constructor  *)
+        constr_trees <- except (IndexErr "build_recargs_nested/mk_ind_recargs" "no tree for inductive" j) $ 
+          nth_error trees j;;
+        arg_trees <- except (IndexErr "build_recargs_nested/mk_ind_recargs" "no tree for constructor" k) $ 
+          nth_error constr_trees k;; 
+        (* recursively build the trees for the constructor's arguments, potentially traversing nested inductives *)
+        build_recargs_constructors Σ Γ' ra_env' arg_trees c'
+      ) abstracted_constrs;;
+      (* make the tree for this nested inductive *)
+      ret $ mk_ind_paths (Imbr (mkInd ind.(inductive_mind) j)) paths
+  in
+  (* create the trees for all the bodies *)
+  ind_recargs <- unwrap $ mapi mk_ind_recargs mib.(ind_bodies);;
+  (* now, given the bodies, make the mutual inductive trees *)
+  trees <- except (OtherErr "build_recargs_nested" "creating trees failed") $ mk_rec ind_recargs;;
+  (* return the tree for our particular inductive type *)
+  tree_ind <- except (IndexErr "build_recargs_nested" "created trees malformed" ind.(inductive_ind)) $ 
+    nth_error trees ind.(inductive_ind);;
+  ret tree_ind)
+
+(** Build the recargs tree for a term [t] -- in practice, [t] will be the type of a constructor argument. *)
+(* In the case that [t] contains nested inductive calls, [tree] is used to decide when to traverse nested inductives. *)
+(* [ra_env] is used to keep track of the subterm information of dB variables. 
+   It need not bind all variables occurring in [t]: to unbound indices, we implicitly assign [Norec].*)
+(* This code is very close to check_positive in indtypes.ml, but does no positivity check and does not compute the number of recursive arguments. *)
+(* In particular, this code handles nested inductives as described above. *)
+with build_recargs Σ Γ (ra_env : list (recarg * wf_paths)) (tree : wf_paths) (t : term) {struct t}: exc wf_paths := 
+  t_whd <- whd_all Σ Γ t;;
+  let '(x, args) := decompose_app t_whd in
+  match x with 
+  | tProd na type body => 
+      (* simply enter the prod, adding the quantified element as assumption of non-recursive type (even though the type may in fact be inductive, for the purpose of determining the recargs tree of [t], this is irrelevant)*)
+      assert (args == []) (OtherErr "build_recargs" "tProd case: term is ill-typed");;
+      let Γ' := Γ ,, vass na type in
+      let ra_env' := (Norec, mk_norec) :: ra_env in
+      build_recargs Σ Γ' ra_env' tree body
+  | tRel k => 
+      (* free variables are allowed and assigned Norec *)
+      catchE (k_ra <- except (OtherErr "" "") $ nth_error ra_env k;; ret (snd k_ra)) 
+            (fun _ => ret mk_norec)
+  | tInd ind _ => 
+    (* if the given tree for [t] allows it (i.e. has an inductive as label at the root), we traverse a nested inductive *)
+    match destruct_recarg tree with 
+    | None => raise $ OtherErr "build_recargs" "tInd case: malformed recargs tree"
+    | Some (Imbr ind') | Some (Mrec ind') => 
+        if ind == ind' then build_recargs_nested Σ Γ ra_env tree ind args 
+                       else ret mk_norec
+    | _ => ret mk_norec 
+    end
+  | _ => ret mk_norec
+  end
+
+  
+
+(* [build_recargs_constructors Σ Γ ra_env trees c] builds a list of each of the constructor [c]'s argument's recursive structures, instantiating nested inductives suitably.  
+  We assume that [c] excludes parameters -- these should already be contained in the environment. 
+
+  [trees] is a list of trees for the constructor's argument types, used to determine when to traverse nested inductive types.
+
+  [ra_env] is used to keep track of the recursive trees of dB variables. 
+   It need not bind all variables occurring in [t]: to unbound indices, we implicitly assign [Norec] with a trivial recursive tree.
+*)
+with build_recargs_constructors Σ Γ (ra_env : list (recarg * wf_paths)) (trees : list wf_paths) (c : term) {struct c}: exc (list wf_paths) := 
+  let recargs_constr_rec := fix recargs_constr_rec Γ (ra_env : list (recarg * wf_paths)) (trees : list wf_paths) (lrec :list wf_paths) (c : term) {struct c} : exc (list wf_paths) := 
+    c_whd <- whd_all Σ Γ c;;
+    let '(x, args) := decompose_app c_whd in
+    match x with 
+    | tProd na type body => 
+        (* the constructor has an argument of type [type] *)
+        assert (args == []) (OtherErr "build_recargs_constructors" "tProd case: ill-typed term");;
+        (* compute the recursive structure of [type] *)
+        first_tree <- except (ProgrammingErr "build_recargs_constructors" "trees is too short") $
+          hd trees;;
+        rec_tree <- build_recargs Σ Γ ra_env first_tree type;;
+        (* [na] of type [type] can be assumed to be of non-recursive type for this purpose *)
+        let Γ' := Γ ,, vass na type in
+        let ra_env' := (Norec, mk_norec) :: ra_env in 
+        (* process the rest of the constructor type *)
+        rest_trees <- except (OtherErr "build_recargs_constructors" "trees list too short") $ 
+          tl trees;;
+        recargs_constr_rec Γ' ra_env' rest_trees (rec_tree :: lrec) body
+    | _ => 
+        (* we have processed all the arguments of the constructor -- reverse to get a valid dB-indexed context *)
+        ret $ rev lrec  
+    end
+  in recargs_constr_rec Γ ra_env trees [] c. 
+
+
+(* [get_recargs_approx env tree ind args] builds an approximation of the recargs
+tree for [ind], knowing [args] that are applied to it. 
+The argument [tree] is used to know when candidate nested types should be traversed, pruning the tree otherwise. *)
+Definition get_recargs_approx Σ Γ (tree : wf_paths) (ind : inductive) (args : list term) : exc wf_paths := 
+  (* starting with ra_env = [] seems safe because any unbound tRel will be assigned Norec *)
+  build_recargs_nested Σ Γ [] tree ind args. 
+
+
+(* [restrict_spec_for_match Σ Γ spec rtf] restricts the size information in [spec] to what is allowed to flow through a match with return-type function (aka predicate) [rtf] in environment (Σ, Γ). *)
+(* [spec] is the glb of the subterm specs of the match branches*)
+(* (this is relevant for cases where we go into recursion with the result of a match) *)
+(* TODO: how does get_recargs_approx play into this?*)
 Definition restrict_spec_for_match Σ Γ spec (rtf : term) : exc subterm_spec := 
   if spec == Not_subterm then ret Not_subterm
   else 
@@ -989,52 +841,79 @@ Definition restrict_spec_for_match Σ Γ spec (rtf : term) : exc subterm_spec :=
   if negb(rel_range_occurs 0 (length rtf_context - 1) rtf) then ret spec 
   else
     (* decompose the rtf into context and rest and check if there is an inductive at the head *)
-    let Γ' := rtf_context ++ Γ in
+    let Γ' := Γ ,,, rtf_context in
     '(rtf_context', rtf') <- decompose_prod_assum Σ Γ rtf;;
-    let Γ'' := rtf_context' ++ Γ' in
+    let Γ'' := Γ' ,,, rtf_context' in
     rtf'_whd <- whd_all Σ Γ rtf';;
     let '(i, args) := decompose_app rtf'_whd in 
     match i with 
-    | tInd ind univ => (* there's an inductive [ind] at the head under the lambdas, prods, and lets *)
+    | tInd ind _ => (* there's an inductive [ind] at the head under the lambdas, prods, and lets *)
         match spec with 
         | Dead_code => ret Dead_code
         | Subterm size tree => 
             (* intersect with approximation obtained by unfolding *)
+            (* TODO: when does get_recargs_approx actually do something other than identity? *)
             recargs <- get_recargs_approx Σ Γ tree ind args;;
-            recargs <- except "restrict_spec_for_match: intersection failed" $ inter_wf_paths tree recargs;;
+            recargs <- except (OtherErr "restrict_spec_for_match" "intersection failed") $ inter_wf_paths tree recargs;;
             ret (Subterm size recargs)
-        | _ => raise "this should not be reachable" (* TODO why *)
+        | _ => (* we already caught this case above *)
+            raise $ OtherErr "restrict_spec_for_match" "this should not be reachable" 
         end
     | _ => ret Not_subterm
     end.
 
-(* check if a (function) type has an inductive co-domain *)
-Definition has_inductive_codomain Σ Γ t : exc bool := 
-  '(abs_context, t') <- decompose_lam_assum Σ Γ t;;
-  let Γ' := abs_context ++ Γ in
-  '(context', t'') <- decompose_prod_assum Σ Γ t';;
-  let Γ'' := context' ++ Γ' in
-  t''_whd <- whd_all Σ Γ'' t'';;
-  let '(i, _) := decompose_app t''_whd in
-  match i with 
-  | tInd _ _ => ret true
-  | _ => ret false 
-  end.
+
+(** ** Checking fixpoints *)
 
 
-Definition lookup_ind_subterms Σ (ind : inductive) :=
-  '(_, oib) <- lookup_mind_specif Σ ind;;
-  ret oib.(ind_recargs).
+(* Given a subterm spec for a term to match on, compute the subterm specs for the binders bound by a match in the individual branches. *)
+(* In [match c as z in ci y_s return P with |C_i x_s => t end]
+   [branches_specif Σ G c_spec ind] returns a list of [x_s]'s specs knowing
+   [c_spec]. *)
+(* [ind] is the inductive we match on. *)
+Definition branches_binders_specif Σ G (discriminant_spec : subterm_spec) (ind : inductive) : exc list (list subterm_spec) := 
+  (* get the arities of the constructors (without lets, without parameters) *)
+  constr_arities <- (
+    '(_, oib) <- lookup_mind_specif Σ ind;;
+    ret $ map snd oib.(ind_ctors));;
+  unwrap $ mapi (fun i (ar : nat) => 
+    match discriminant_spec return exc (list subterm_spec)  with 
+    | Subterm _ tree => 
+        (* check if the tree refers to the same inductive as we are matching on *)
+        recarg_info <- except (OtherErr "branches_binders_specif" "malformed tree") $ destruct_recarg tree;;
+        if negb (match_recarg_inductive ind recarg_info) then
+          (* the tree talks about a different inductive than we are matching on, so all the constructor's arguments cannot be subterms  *)
+          ret $ tabulate (fun _ => Not_subterm) ar
+        else 
+          (* get trees for the arguments of the i-th constructor *)
+          constr_args_sizes <- wf_paths_constr_args_sizes tree;;
+          args_sizes <- except (IndexErr "branches_binders_specif" "no tree for constructor" i) $
+            nth_error constr_args_sizes i;;
+          (* this should hopefully be long enough and agree with the arity of the constructor *)
+          assert (length args_sizes == ar) (OtherErr "branches_binders_specif" "number of constructor arguments don't agree");;
+          (* for each arg of the constructor: generate a strict subterm spec if they are recursive, otherwise Not_subterm. 
+            These do also contain the recursive tree for that argument to enable nested matches. *)
+          ret $ map spec_of_tree args_sizes 
+    | Dead_code => 
+        (* just propagate *)
+        ret $ tabulate (fun _ => Dead_code) ar
+    | Not_subterm => 
+        (* just propagate *)
+        ret $ tabulate (fun _ => Not_subterm) ar
+    end
+    ) constr_arities.
 
-(* FIXME: is not structurally recursive *)
-(* [subterm_specif Σ G stack t] computes the recursive structure of [t] applied to elements with the subterm structures given by the [stack]. 
+
+(* [subterm_specif Σ G stack t] computes the recursive structure of [t] applied to arguments with the subterm structures given by the [stack]. 
   [G] collects subterm information about variables which are in scope. 
 *)
 Fixpoint subterm_specif Σ G (stack : list stack_element) t {struct t}: exc subterm_spec:= 
   t_whd <- whd_all Σ G.(loc_env) t;;
   let '(f, l) := decompose_app t_whd in 
   match f with 
-  | tRel k => ret $ lookup_subterm G k
+  | tRel k => 
+      (* we abstract from applications: if [t] is a subterm, then also [t] applied to [l] is a subterm *)
+      ret $ lookup_subterm G k
   | tCase ind_relev rtf discriminant branches => 
       let '(ind, relev) := ind_relev in
       (* push l to the stack *)
@@ -1044,22 +923,23 @@ Fixpoint subterm_specif Σ G (stack : list stack_element) t {struct t}: exc subt
       (* get subterm info for the binders in the branches *)
       branches_binders_specs <- branches_binders_specif Σ G discriminant_spec (fst ind);;
       (* determine subterm info for the full branches *)
-      branches_specs <- exc_unwrap $ mapi (fun i branch => 
-        binder_specs <- except "" $ nth_error branches_binders_specs i;;
+      branches_specs <- unwrap $ mapi (fun i branch => 
+        binder_specs <- except (IndexErr "subterm_specif" "branches_binders_specif result is too short" i) $ 
+          nth_error branches_binders_specs i;;
         let stack_br := push_stack_args stack' binder_specs in
         subterm_specif Σ G stack_br branch) (map snd branches);;
-      (* take their glb *)
+      (* take their glb -- in case of no branches, this yields [Dead_code] (absurd elimination) *)
       spec <- subterm_spec_glb branches_specs;;
       (* restrict the subterm info according to the rtf *)
       restrict_spec_for_match Σ G.(loc_env) spec rtf 
   | tFix mfix mfix_ind => 
-      cur_fix <- except "invalid fixpoint index" $ nth_error mfix mfix_ind;;
+      cur_fix <- except (IndexErr "subterm_specif" "invalid fixpoint index" mfix_ind) $ nth_error mfix mfix_ind;;
       (* if the co-domain isn't an inductive, this surely can't be a subterm *)
       ind_cod <- (has_inductive_codomain Σ G.(loc_env) cur_fix.(dtype));; 
       if negb ind_cod then ret Not_subterm 
       else 
         '(context, cur_fix_codomain) <- decompose_prod Σ G.(loc_env) cur_fix.(dtype);;
-        let Γ' := context ++ G.(loc_env) in 
+        let Γ' := G.(loc_env) ,,, context in 
         (* if we can't find the inductive, it is not a subterm. *)
         (* TODO is there actually a case where this is valid behvaviour? *)
         catchMap (find_inductive Σ Γ' cur_fix_codomain) (fun _ => ret Not_subterm) $ fun '((ind, _), _) => 
@@ -1085,22 +965,22 @@ Fixpoint subterm_specif Σ G (stack : list stack_element) t {struct t}: exc subt
         (* before we go on to check the body: if there are enough arguments on the stack, 
           we can use the subterm information on the stack for the decreasing argument of 
           the nested fixpoint (instead of taking Not_subterm) *)
-        (* we check the body with an empty stack *)
+        (* we check the body with an empty stack as it isn't directly applied to something*)
         if Nat.ltb (length stack') num_abstractions then subterm_specif Σ G'' [] body' else
-          decreasing_arg_stackel <- except "" $ nth_error stack' decreasing_arg;;
+          decreasing_arg_stackel <- except (IndexErr "subterm_specif" "stack' too short" decreasing_arg) $ 
+            nth_error stack' decreasing_arg;;
           arg_spec <- stack_element_specif Σ decreasing_arg_stackel;;
           let G'' := update_guard_spec G'' 0 arg_spec in 
           subterm_specif Σ G'' [] body'
   | tLambda x ty body => 
-     assert (l == []) "reduction is broken";;
-     (* get the subterm spec of what the lambda would be applied to *)
-     (* TODO: why don't we need to check for emptiness here?*)
+     assert (l == []) (OtherErr "subterm_specif" "reduction is broken");;
+     (* get the subterm spec of what the lambda would be applied to (or Not_subterm if [stack] is empty)*)
      '(spec, stack') <- extract_stack_hd Σ stack;;
      subterm_specif Σ (push_guard_env G (x, ty, spec)) stack' body 
   | tEvar _ _ => 
       (* evars are okay *)
-      (* TODO: check handling of Dead_code at other places *)
-      ret Dead_code
+      (*ret Dead_code*)
+      raise $ OtherErr "subterm_specif" "the guardedness checker does not handle evars"
   | tProj p t => 
       (* compute the spec for t *)
       (* TODO: why do we do this with the stack (instead of the empty stack)?
@@ -1113,10 +993,11 @@ Fixpoint subterm_specif Σ G (stack : list stack_element) t {struct t}: exc subt
           | [arg_tree] => 
               (* get the tree of the projected argument *)
               let proj_arg := snd p in
-              proj_arg_tree <- except "malformed recursive tree" $ nth_error arg_tree proj_arg;;
+              proj_arg_tree <- except (IndexErr "subterm_specif" "malformed recursive tree" proj_arg) $ 
+                nth_error arg_tree proj_arg;;
               (* make a spec out of it *)
               ret (spec_of_tree proj_arg_tree)
-          | _ => raise "projection on type having a number of constructors ≠ 1"
+          | _ => raise $ OtherErr "subterm_specif" "projection on type having a number of constructors ≠ 1"
           end
       | Dead_code => ret Dead_code
       | Not_subterm => ret Not_subterm
@@ -1140,15 +1021,15 @@ with extract_stack_hd Σ stack {struct stack} : exc (subterm_spec * list stack_e
       ret (spec, stack)
   end.
 
-Set Guard Checking.
-
 (* Check that a term [t] with subterm spec [spec] can be applied to a fixpoint whose recursive argument has subterm structure [tree]*)
 Definition check_is_subterm spec tree := 
   match spec with 
   | Subterm Strict tree' => 
       (* TODO: find an example where the inclusion checking is needed -- probably with nested inductives? *)
       incl_wf_paths tree tree'
-  | Dead_code => true
+  | Dead_code => 
+      (* [spec] been constructed by elimination of an empty type, so this is fine *)
+      true
   | _ => false
   end.
 
@@ -1180,16 +1061,16 @@ Definition filter_stack_domain Σ Γ (rtf : term) (stack : list stack_element) :
   if negb (rel_range_occurs 0 (length rtf_context -1) rtf_body) then ret stack 
   else
     (* enter the rtf context *)
-    let Γ' := rtf_context ++ Γ in
+    let Γ' := Γ ,,, rtf_context in
     let filter_stack := fix filter_stack Γ t stack : exc (list stack_element) := 
       t' <- whd_all Σ Γ t;;
       match stack, t' with 
       | elem :: stack', tProd na ty t0 => 
-        (* the element elem in the stack would be applied to what corresponds to the ∀ na : ty, t0 in the rtf *)
+        (* the element [elem] in the stack would be applied to what corresponds to the [∀ na : ty, t0] in the rtf *)
         let d := vass na ty in 
         (* decompose the type [ty] of [na] *)
         '(ctx, ty) <- decompose_prod_assum Σ Γ ty;;
-        let Γ' := ctx ++ Γ in
+        let Γ' := Γ ,,, ctx in
         (* now in the context of the type *)
         whd_ty <- whd_all Σ Γ' ty;;
         (* decompose the rest of the type again and check if the LHS is an inductive *)
@@ -1204,8 +1085,10 @@ Definition filter_stack_domain Σ Γ (rtf : term) (stack : list stack_element) :
               | Not_subterm | Dead_code => ret elem (* don't restrict *)
               | Subterm s path => 
                   (* intersect with an approximation of the unfolded tree for [ind] *)
+                  (* TODO : when does get_recargs_approx give something other than identity ? *)
                   recargs <- get_recargs_approx Σ Γ path ind ty_args;;
-                  path' <- except "intersection of trees failed" $  inter_wf_paths path recargs;;
+                  path' <- except (OtherErr "filter_stack_domain" "intersection of trees failed") $ 
+                    inter_wf_paths path recargs;;
                   (* update the recargs tree to [path'] *)
                   ret $ SArg (Subterm s path') 
               end
@@ -1220,16 +1103,6 @@ Definition filter_stack_domain Σ Γ (rtf : term) (stack : list stack_element) :
       end
     in filter_stack Γ' rtf_body stack.
 
-From ReductionEffect Require Import PrintingEffect. 
-  (*Fixpoint test (n : nat) := *)
-    (*match n with *)
-    (*| 0 => 0 *)
-    (*| S n => print_id (S (test n))*)
-    (*end.*)
-  (*Eval cbn in (test 4).*)
-
-Definition print {A} (a : A) : exc A := ret (print_id a). 
-
 (* 
   The main checker descending into the recursive structure of a term.
   Checks if [t] only makes valid recursive calls, with variables (and their subterm information) being tracked in the context [G].
@@ -1238,8 +1111,6 @@ Definition print {A} (a : A) : exc A := ret (print_id a).
   For example: for the term [(match .. with |.. => t end) u], [t] will be checked with (the subterm information of) [u] on the stack. This is needed as we (of course) might not be able to reduce the match, but still want to be able to reason about [t] being applied to [u] after reduction.
 
   [trees] is the list of recursive structures for the decreasing arguments of the mutual fixpoints.*)
-(* FIXME: make structurally recursive *)
-Unset Guard Checking. 
 Fixpoint check_rec_call (num_fixes : nat) (decreasing_args : list nat) trees
 Σ G (stack : list stack_element) (t : term) {struct t} : exc unit := 
   let check_rec_call' := check_rec_call num_fixes decreasing_args trees Σ in 
@@ -1259,26 +1130,42 @@ Fixpoint check_rec_call (num_fixes : nat) (decreasing_args : list nat) trees
           (* get the position of the invoked fixpoint in the mutual block *)
           let rec_fixp_index := G.(rel_min_fix) + num_fixes -1 - p in
           (* get the decreasing argument of the recursive call *)
-          decreasing_arg <- except "check_rec_call: invalid fixpoint index" $ nth_error decreasing_args rec_fixp_index;;
+          decreasing_arg <- except (IndexErr "check_rec_call" "invalid fixpoint index" rec_fixp_index) $ 
+            nth_error decreasing_args rec_fixp_index;;
           (* push the arguments as closures on the stack -- we don't infer their full subterm information yet *)
-          (* TODO : we don't really need to construct the updated stack here! *)
+          (* NOTE : we don't really need to construct the updated stack here, but it seems cleaner *)
           let stack' := push_stack_closures G stack l in 
           (* get the stack entry for the decreasing argument *)
-          z <- except "check_rec_call: not enough arguments for recursive fix call" $ nth_error stack' decreasing_arg;;
+          z <- except (IndexErr "check_rec_call" "not enough arguments for recursive fix call" decreasing_arg) $ 
+            nth_error stack' decreasing_arg;;
           (* get the tree for the recursive argument type *)
-          recarg_tree <- except "check_rec_call: no tree for the recursive argument" $ nth_error trees rec_fixp_index;;
+          recarg_tree <- except (IndexErr "check_rec_call" "no tree for the recursive argument" rec_fixp_index) $ 
+            nth_error trees rec_fixp_index;;
           (* infer the subterm spec of the applied argument *)
           rec_subterm_spec <- stack_element_specif Σ z;;
           (* verify that it is a subterm *)
           if negb (check_is_subterm rec_subterm_spec recarg_tree) 
           then 
             match z with 
-            | SClosure z z' => raise "illegal recursive call (could not ensure that argument is decresasing)"
-            | SArg _ => raise "check_rec_call: fix was partially applied"
+            | SClosure z z' => raise $ GuardErr "check_rec_call" "illegal recursive call (could not ensure that argument is decresasing)"
+            | SArg _ => 
+                (* TODO: check if this is the right error *)
+                raise $ GuardErr "check_rec_call" "fix was partially applied"
             end
           else ret tt
         else ret tt
 
+    (* Assume we are checking the fixpoint f. For checking [g a1 ... am]:
+      if - g = match d return rtf with | Ci xi1 ... xin => bi end
+         - f is guarded with respect to the set of subterms S in a1 ... am
+         - f is guarded with respect to the set of subterms S in the return-type function rtf
+         - f is guarded with respect to the set of subterms S in the discriminant d
+         - for each branch Ci xi1 ... xin => bi where S' := S ∪ { xij | the constructor Ci is recursive in the argument xij }:
+            f is guarded with respec to S' in the branch body
+            bi (virtually) applied to a1 ... am, where we restrict the subterm information of a1 ... am to 
+            what is allowed to flow through the rtf
+      then f is guarded with respect to the set of subterms S in [g a1 ... am].
+    *)
     | tCase ind_nparams_relev rtf discriminant branches => 
         (* match discriminant : ind return rtf with [branches] end *)
         let '((ind, nparams), relev) := ind_nparams_relev in
@@ -1288,7 +1175,7 @@ Fixpoint check_rec_call (num_fixes : nat) (decreasing_args : list nat) trees
           _ <- list_iter (check_rec_call' G []) l;;
           _ <- check_rec_call' G [] rtf;;
           _ <- check_rec_call' G [] discriminant;;
-          (* compute the recursive argument info for the arguments of each branch by looking at the tree *)
+          (* compute the recursive argument info for the binders of each branch by looking at the tree *)
           discriminant_spec <- subterm_specif Σ G [] discriminant;; 
           case_branch_specs <- branches_binders_specif Σ G discriminant_spec ind;; 
           (* push arguments on stack *)
@@ -1297,8 +1184,9 @@ Fixpoint check_rec_call (num_fixes : nat) (decreasing_args : list nat) trees
           stack' <- filter_stack_domain Σ G.(loc_env) rtf stack';;
           (* check the branches of the matches *)
           list_iteri (fun i '(_, branch) =>
-              branch_spec <- except "check_rec_call: branch specs too short" $ nth_error case_branch_specs i;;
-              (* NOTSURE push the rec arg specs for the variables introduced by the branch *)
+              branch_spec <- except (IndexErr "check_rec_call" "branch specs too short" i) $ 
+                nth_error case_branch_specs i;;
+              (* push the rec arg specs for the binders introduced by the branch *)
               let stack_branch := push_stack_args stack' branch_spec in
               (* check the branch *)
               check_rec_call' G stack_branch branch) 
@@ -1315,20 +1203,16 @@ Fixpoint check_rec_call (num_fixes : nat) (decreasing_args : list nat) trees
           | _ => raise err
           end)
 
-    (* Enables to traverse Fixpoint definitions in a more intelligent
-       way, ie, the rule :
-       if - g = fix g (y1:T1)...(yp:Tp) {struct yp} := e &
-          - f is guarded with respect to the set of pattern variables S
-            in a1 ... am        &
-          - f is guarded with respect to the set of pattern variables S
-            in T1 ... Tp        &
-          - ap is a sub-term of the formal argument of f &
-          - f is guarded with respect to the set of pattern variables
-            S+{yp} in e
-       then f is guarded with respect to S in (g a1 ... am).
-       Eduardo 7/9/98 *)
+    (* Assume we are checking the fixpoint f. 
+       This implements the following rule for checking the term [g a1 ... am]:
+       if - g = fix g (y1:T1)...(yp:Tp) {struct yp} := e 
+          - f is guarded with respect to the set of subterms S in a1 ... am        
+          - f is guarded with respect to the set of subterms S in T1 ... Tp        
+          - ap is a sub-term of the recursive argument of f and f is guarded with respect to the set of subterms S ∪ {yp} in e
+           OR ap is not a sub-term of the recursive argument of f and f is guarded with respect to the set of subterms S in e
+       then f is guarded with respect to the set of subterms S in (g a1 ... am). *)
     | tFix mfix_inner fix_ind => 
-        this_fix <- except "malformed fixpoint" $ nth_error mfix_inner fix_ind;;
+        this_fix <- except (OtherErr "check_rec_call" "tFix: malformed fixpoint") $ nth_error mfix_inner fix_ind;;
         let decreasing_arg := rarg this_fix in 
         catchE (
           (* check args *)
@@ -1342,7 +1226,8 @@ Fixpoint check_rec_call (num_fixes : nat) (decreasing_args : list nat) trees
           list_iteri (fun j body => 
             if (fix_ind == j) && Nat.ltb decreasing_arg (length stack') then
               (* we have subterm information for the decreasing arg on the stack *)
-              rec_arg_stackel <- except "should be unreachable" $ nth_error stack' decreasing_arg;; 
+              rec_arg_stackel <- except (ProgrammingErr "check_rec_call" "should be unreachable") $ 
+                nth_error stack' decreasing_arg;; 
               (* compute the subterm spec for the recursive argument *)
               rec_arg_spec <- stack_element_specif Σ rec_arg_stackel;;
               (* check the body of the fix after entering under the arguments and adding rec_arg_spec as the specification for [decreasing_arg] *)
@@ -1354,7 +1239,8 @@ Fixpoint check_rec_call (num_fixes : nat) (decreasing_args : list nat) trees
           $ fun err => 
             (* try to reduce the fix away by looking for a constructor in l[decreasing_arg] *)
             if Nat.leb (length l) decreasing_arg then raise err else
-            rec_arg_term <- except "should be unreachable" $ nth_error l decreasing_arg;;
+            rec_arg_term <- except (ProgrammingErr "check_rec_call" "should be unreachable") $ 
+              nth_error l decreasing_arg;;
             rec_arg_term <- whd_all Σ G.(loc_env) rec_arg_term;;
             let '(hd, _) := decompose_app rec_arg_term in 
             match hd with 
@@ -1371,26 +1257,32 @@ Fixpoint check_rec_call (num_fixes : nat) (decreasing_args : list nat) trees
           (* check the arguments *)
           catchE (list_iter (check_rec_call' G []) l) $ fun _ => 
           (* an error occurred, maybe it goes better if we apply the arguments reduce the constant? *)
-            val <- except "constant lookup failed, this is weird :(" $ get_const_value Σ kname;;
+            val <- except (ProgrammingErr "check_rec_call" "constant lookup failed") $ get_const_value Σ kname;;
             check_rec_call' G stack (tApp val l)
         else 
           (* just check the arguments without fallback *)
           list_iter (check_rec_call' G []) l
 
+    (* Assume we are checking f. This implements the following rule for checking [g a1 ... an]:
+       if - g = λ x : t. b 
+          - f is guarded wrt the set of subterms S in t
+          - if f is guarded wrt the set of subterms S ∪ { 
+            TODO
+    *) 
     | tLambda x ty body =>
         (* l is empty or reduction is broken *)
-        _ <- assert (l == []) "tLambda : l should be empty";;
+        _ <- assert (l == []) (OtherErr "check_rec_call" "tLambda : reduction is broken");;
         (* check the type *)
         check_rec_call' G [] ty;;
-        (* we take the subterm spec at the head of the stack (corresponding to the element which will be applied to this lambda)*)
+        (* we take the subterm spec at the head of the stack (corresponding to the element which will be applied to this lambda), or No_subterm if the stack is empty *)
         '(spec, stack') <- extract_stack_hd Σ stack;;
         (* and check the body in the updated environment with the spec for this applied element *)
         check_rec_call' (push_guard_env G (x, ty, spec)) stack' body
 
 
     | tProd x ty body => 
-        (* the list [l] should be empty, otherwise reduction is broken *)
-        _ <- assert (l == []) "tProd: l should be empty";;
+        (* the list [l] should be empty, otherwise the term is ill-typed *)
+        _ <- assert (l == []) (OtherErr "check_rec_call" "tProd: input term is ill-typed");;
         (* moreover, the stack should be empty: 
           We only ever put elements on the stack when we cannot reduce a match. 
           Arguments which would be applied to a Prod would however not be allowed to flow through a match. 
@@ -1436,17 +1328,18 @@ Fixpoint check_rec_call (num_fixes : nat) (decreasing_args : list nat) trees
     | tVar id => 
         (* FIXME: environments for named variables do not seem to be properly implemented in MetaCoq.
           However, I think they are only ever used for section variables in Coq, I believe. *)
-        raise "handling of named variables is unimplemented"
+        raise (ProgrammingErr "check_rec_call" "handling of named variables is unimplemented")
 
     | tSort _ => 
         (* a sort shouldn't be applied to anything; guardedness is fine of course *)
-        assert (l == []) "sorts shouldn't be applied to anything..."
+        assert (l == []) $ OtherErr "check_rec_call" "tSort: ill-typed term"
 
     | tEvar _ _ => 
         (* the RHS [l] is not checked because it is considered as the evar's context *)
-        (* TODO : is that really okay? *)
-        ret tt
-    | tApp _ _ | tLetIn  _ _ _ _ | tCast _ _ _ => raise "beta-zeta-iota reduction is broken"
+        (* NOTE: the guard checker is not really supposed to be dealing with evars -- it should be called on evar-free terms;
+          see https://github.com/coq/coq/issues/9333#issuecomment-453235650*)
+        raise $ OtherErr "check_rec_call" "guard checker should not be called on terms containing evars"
+    | tApp _ _ | tLetIn  _ _ _ _ | tCast _ _ _ => raise (OtherErr "check_rec_call" "beta-zeta-iota reduction is broken")
     end
 
 (* Check the body [body] of a nested fixpoint with decreasing argument [decr] (dB index) and subterm spec [sub_spec] for the recursive argument.*)
@@ -1468,26 +1361,96 @@ with check_nested_fix_body (num_fixes : nat) (decreasing_args : list nat) trees
         let G' := push_nonrec_guard_env G (x, ty) in  
         check_nested_fix_body num_fixes decreasing_args trees Σ G' n sub_spec body
       end
-  | _ => raise "illformed inner fix body"
+  | _ => raise $ OtherErr "check_nested_fix_body" "illformed inner fix body"
   end.
-Set Guard Checking. 
 
 (* Check if [def] is a guarded fixpoint body, with arguments up to (and including)
   the recursive argument being introduced in the context [G]. 
   [G] has been initialized with initial guardedness information on the recursive argument.
   [trees] is a list of recursive structures for the decreasing arguments of the mutual fixpoints.
-  [recpos] is a list with the recursive argument indicese of the mutually defined fixpoints.
+  [recpos] is a list with the recursive argument indices of the mutually defined fixpoints.
 *)
 Definition check_one_fix Σ G (recpos : list nat) (trees : list wf_paths) (def : term) : exc unit := 
   check_rec_call (length recpos) recpos trees Σ G [] def.  
 
 
+(* Extract the [inductive] that [fixp] is doing recursion over (and check that the recursion is indeed over an inductive).
+  Moreover give the body of [fixp] after the recursive argument and the environment (updated from [Γ])
+  that contains the arguments up to (and including) the recursive argument (of course also the fixpoints). *)
+Definition inductive_of_mutfix Σ Γ (fixp : mfixpoint term) : exc (list inductive * list (context * term)):= 
+  trace "inductive_of_mutfix : enter";;
+  let number_of_fixes := length fixp in
+  assert (number_of_fixes != 0) (OtherErr "inductive_of_mutfix" "ill-formed fix");;
+  let ftypes := mfix_types fixp in
+  let fnames := mfix_names fixp in 
+  let fbodies := mfix_bodies fixp in
+  (* push fixpoints to environment *)
+  let Γ_fix := push_assumptions_context (fnames, ftypes) Γ in
+  let nvect := map rarg fixp in 
+
+  (* Check the i-th definition [fixdef] of the mutual inductive block where k is the recursive argument, 
+    making sure that no invalid recursive calls are in the types of the first [k] arguments, 
+    make sure that the recursion is over an inductive type, 
+    and return that inductive together with the body of [fixdef] after the recursive arguement
+    together with its context. *)
+  let find_ind i k fixdef : exc (inductive * (context * term)):= 
+      (* check that a rec call to the fixpoint [fixdef] does not appear in the [k] first abstractions,
+        that the recursion is over an inductive, and 
+        gives the inductive and the body + environment of [fixdef] after introducing the first [k] arguments *)
+      let check_occur := fix check_occur Γ n (def : term) {struct def}: exc (inductive * (context * term)) := 
+        (* n is the number of lambdas we're under/aka the dB from which the mutual fixes are starting:
+          n ... n + number_of_fixes - 1 *)
+        def_whd <- whd_all Σ Γ def;;
+        match def_whd with 
+        | tLambda x t body => 
+            assert (negb(rel_range_occurs n number_of_fixes t)) 
+              (GuardErr "inductive_of_mutfix" "bad occurrence of recursive call");;
+            let Γ' := Γ ,, (vass x t) in
+            if n == k then (* becomes true once we have entered [k] inner lambdas*)
+              (* so now the rec arg should be at dB 0 and [t] is the type we are doing recursion over *)
+              (* get the inductive type of the fixpoint, ensuring that it is an inductive *)
+              '((ind, _), _) <- catchE (find_inductive Σ Γ t) (fun _ => raise $ GuardErr "inductive_of_mutfix" "recursion not on inductive");;
+              '(mib, _) <- lookup_mind_specif Σ ind;;
+              if mib.(ind_finite) != Finite then (* ensure that it is an inductive *)
+                raise $ GuardErr "inductive_of_mutfix" "recursion not on inductive"
+              else
+                (* now return the inductive, the env after taking the inductive argument and all arguments before it, and the rest of the fix's body *)
+                ret (ind, (Γ', body))
+            else check_occur Γ' (S n) body
+        | _ => 
+            (* not a lambda -> we do not have enough arguments and can't find the recursive one *)
+            raise $ GuardErr "inductive_of_mutfix" "not enough abstractions in fix body" 
+        end
+      in 
+      (* check that recursive occurences are nice and extract inductive + fix body *)
+      res <- check_occur Γ_fix 0 fixdef;; 
+      let '(ind, _) := res in
+      '(_, oib) <- lookup_mind_specif Σ ind;;
+      (*if oib.(ind_relevance) == Irrelevant && *)
+      (* TODO some sprop checking for relevance *)
+      ret res
+  in 
+  (* now iterate this on all the fixpoints of the mutually recursive block *)
+  rv <- unwrap $ map2_i find_ind nvect fbodies;;
+  trace "inductive_of_mutfix : leave";;
+  (* return the list of inductives as well as the fixpoint bodies in their context *)
+  ret (map fst rv : list inductive, map snd rv : list (context * term)).
+
+
+
+
+(* The entry point for checking fixpoints. 
+  [Σ]: the global environment with all definitions used in [mfix]. 
+  [Γ]: the local environment in which the fixpoint is defined.
+  [mfix]: the fixpoint to check.
+*)
 Definition check_fix Σ Γ (mfix : mfixpoint term) : exc unit := 
   (* check that the recursion is over inductives and get those inductives 
     as well as the bodies of the fixpoints *)
+  trace "enter check_fix";;
   '(minds, rec_defs) <- inductive_of_mutfix Σ Γ mfix;;
   (* get the inductive definitions -- note that the mibs should all be the same*)
-  specifs <- exc_unwrap $ map (lookup_mind_specif Σ) minds;;
+  specifs <- unwrap $ map (lookup_mind_specif Σ) minds;;
   let mibs := map fst specifs in
   let oibs := map snd specifs in
   let rec_trees := map (fun oib => oib.(ind_recargs)) oibs in
@@ -1503,10 +1466,10 @@ Definition check_fix Σ Γ (mfix : mfixpoint term) : exc unit :=
   let fix_bodies := map snd rec_defs in   (* the bodies under the respective [fix_envs] *)
   let rec_args := map rarg mfix in 
 
-  _ <- exc_unwrap $ mapi (fun i fix_body => 
-    fix_env <- except "fix_envs too short" $ nth_error fix_envs i;;
-    rec_tree <- except "rec_trees too short" $ nth_error rec_trees i;;
-    rec_arg <- except "rec args too short" $ nth_error rec_args i;;
+  _ <- unwrap $ mapi (fun i fix_body => 
+    fix_env <- except (IndexErr "check_fix" "fix_envs too short" i) $ nth_error fix_envs i;;
+    rec_tree <- except (IndexErr "check_fix" "rec_trees too short" i) $ nth_error rec_trees i;;
+    rec_arg <- except (IndexErr "check_fix" "rec args too short" i) $ nth_error rec_args i;;
     (* initial guard env *)
     let G := init_guard_env fix_env rec_arg rec_tree in
     (* check the one fixpoint *)
@@ -1515,247 +1478,3 @@ Definition check_fix Σ Γ (mfix : mfixpoint term) : exc unit :=
   ret tt.
 
 
-
-
-
-
-
-
-
-
-
-
-
-
-
-
-
-
-
-
-
-
-
-
-
-
-
-
-
-
-
-
-
-
-
-
-
-
-
-
-
-
-
-
-
-
-
-
-
-
-
-
-
-
-
-
-
-From MetaCoq.Template Require Import Environment utils.RTree Ast AstUtils All. 
-Open Scope string_scope.
-Require Import List String.
-Import ListNotations.
-Open Scope string_scope.
-
-Module kernel_lists.
-(* Kernel representation of lists *)
-Definition list_indname : inductive := 
-  {|
-   inductive_mind := (MPfile ["Datatypes"; "Init"; "Coq"], "list");
-   inductive_ind := 0 
-  |}.
-  
-(* NOTE: the constructor arguments in recargs trees are always without lets and without params! *)
-Definition list_recargs : wf_paths := 
-  Rec 0 [ Node (Mrec list_indname) [ Node Norec []; Node Norec [ Node Norec []; 
-                                                                 Param 0 1]
-                                   ]
-        ].
-Eval cbn in (expand (list_recargs)). 
-
-(*Inductive test := *)
-  (*| abc : let a := 10 * 10 in nat -> test. *)
-
-(*Eval hnf in let a := 10 * 10 in nat -> test.*)
-
-(*Print one_inductive_body.*)
-(* I don't really care about universes, just use Set everywhere *)
-
-Definition list_indbody : one_inductive_body := 
-  {| 
-    ind_name := "list";
-    ind_type := tProd {| binder_name := nNamed "A"; binder_relevance := Relevant |}
-                      (tSort (Universe.of_levels (inr (Level.Level "Coq.Init.Datatypes.60"))))
-                      (tSort (Universe.from_kernel_repr (Level.lSet, false) [(Level.Level "Coq.Init.Datatypes.60", false)]));
-    ind_kelim := InType;
-    ind_ctors := [("nil", tProd {|
-                               binder_name := nNamed "A";
-                               binder_relevance := Relevant |}
-                             (tSort
-                                (Universe.of_levels
-                                   (inr
-                                      (Level.Level "Coq.Init.Datatypes.60"))))
-                             (tApp (tRel 1) [tRel 0]), 0);
-                          ("cons",
-                          tProd
-                            {|
-                            binder_name := nNamed "A";
-                            binder_relevance := Relevant |}
-                            (tSort
-                               (Universe.of_levels
-                                  (inr
-                                     (Level.Level "Coq.Init.Datatypes.60"))))
-                            (tProd
-                               {|
-                               binder_name := nAnon;
-                               binder_relevance := Relevant |} 
-                               (tRel 0)
-                               (tProd
-                                  {|
-                                  binder_name := nAnon;
-                                  binder_relevance := Relevant |}
-                                  (tApp (tRel 2) [tRel 1])
-                                  (tApp (tRel 3) [tRel 2]))), 2)];
-               ind_projs := [];
-               ind_relevance := Relevant;
-               ind_recargs := list_recargs |}. 
-
-
-
-(* I don't care about universes. *)
-Definition univdecl := Monomorphic_ctx
-                   (LevelSetProp.of_list
-                      [Level.Level "Coq.Init.Datatypes.60"],
-                   ConstraintSet.empty).
-
-
-Definition list_param_ctxt := 
-[{|
-   decl_name := {|
-                binder_name := nNamed "A";
-                binder_relevance := Relevant |};
-   decl_body := None;
-   decl_type := tSort
-                  (Universe.of_levels
-                     (inr (Level.Level "Coq.Init.Datatypes.60"))) |}].
-Definition list_mindbody : mutual_inductive_body := 
-  {| 
-    ind_bodies := [list_indbody];
-    ind_finite := Finite;
-    ind_npars := 1;
-    (*ind_npars_unif := 1;*)
-    ind_params := list_param_ctxt;
-    ind_universes := univdecl;
-    ind_variance := None;
-  |}.
-
-
-Definition list_entry := (MPfile ["Datatypes"; "Init"; "Coq"], "list", InductiveDecl list_mindbody). 
-
-(*From MetaCoq.Template Require Import Inductives.*)
-
-Require Import List String.
-Import MonadNotation.
-Import ListNotations.
-Open Scope string_scope.
-
-(*Definition list_env. *)
-(* explicit instantiation with TemplateMonad as a definition parametric over the monad causes trouble with universe polymorphism *)
-Definition list_iter {X} (f : X -> TemplateMonad unit) (l : list X) : TemplateMonad unit := 
-  List.fold_left (fun (acc : TemplateMonad unit) x => _ <- acc;; f x) l (ret tt).
-
-
-(* whoops, I've turned the guardedness checker off *)
-Unset Guard Checking.
-Fixpoint broken_app {A : Type} (l m : list A) {struct l} := 
-  match l with
-  | [] => m
-  | a :: l' => broken_app l m
-  end.
-
-Unset Guard Checking.
-(*Set Typeclasses Debug.*)
-(*Check (_ : Monad TemplateMonad). *)
-Fixpoint check_fix_term (Σ : global_env) (Γ : context) (t : term) {struct t} := 
-  match t with 
-  | tFix mfix _ => 
-      (* TODO: we should first recursively check the body of the fix (in case of nested fixpoints!) *)
-      (*tmPrint mfix ;;*)
-      (*tmPrint Σ*)
-      (*ret tt*)
-      (*let Σ := *)
-      catchMap (check_fix Σ Γ mfix) 
-        (fun s => tmPrint s) (fun _ => tmPrint "success")
-  | tCoFix mfix idx =>
-      (* TODO *)
-      ret tt
-  | tLambda na T M => 
-      _ <- check_fix_term Σ Γ T;;
-      _ <- check_fix_term Σ (Γ ,, vass na T) M;;
-      ret tt
-  | tApp u v => 
-      _ <- check_fix_term Σ Γ u;;
-      _ <- list_iter (check_fix_term Σ Γ) v;;
-      ret tt
-  | tProd na A B => 
-      _ <- check_fix_term Σ Γ A;;
-      _ <- check_fix_term Σ (Γ ,, vass na A) B;;
-      ret tt
-  | tCast C kind t => 
-      _ <- check_fix_term Σ Γ C;;
-      _ <- check_fix_term Σ Γ t;;
-      ret tt
-  | tLetIn na b t b' => 
-      _ <- check_fix_term Σ Γ b;;
-      _ <- check_fix_term Σ Γ t;;
-      _ <- check_fix_term Σ (Γ ,, vdef na b t) b';;
-      ret tt
-  | tCase ind rtf discriminant brs =>
-    _ <- check_fix_term Σ Γ rtf;;
-    _ <- check_fix_term Σ Γ discriminant;;
-    _ <- list_iter (fun '(_, b) => check_fix_term Σ Γ b) brs;;
-    ret tt
-  | tProj _ C => 
-      _ <- check_fix_term Σ Γ C;;
-      ret tt
-  | tConst kn u => 
-      match lookup_env_const Σ kn with 
-      | Some const => 
-          match const.(cst_body) with 
-          | Some t => check_fix_term Σ Γ t
-          | _ => ret tt
-          end
-      | None => ret tt
-      end
-  | _ => ret tt 
-      (*tmPrint t;; tmPrint "not a fix" *)
-  end.
-
-Definition check_fix Σ t := check_fix_term Σ [] t. 
-
-
-
-Definition check_fix_start {A} (a : A) :=
-  mlet (Σ, t) <- tmQuoteRec a ;;
-  check_fix (list_entry :: Σ) t.
-MetaCoq Run (check_fix_start broken_app ). 
-MetaCoq Run (check_fix_start app ). 
