guarded/Trace.v
@@ -1,0 +1,114 @@
+From MetaCoq.Template Require Export monad_utils.
+From MetaCoq.Template Require Import utils.
+Export MonadNotation.
+Require Import MetaCoq.Guarded.Except. 
+
+
+Section trace. 
+  Context (max_steps : nat).
+  Context {Y : Type}.
+  Context (timeout : Y). 
+
+  Definition trace_info := string. 
+  Definition TraceM A := nat (* number of steps on the clock *)
+                        * list trace_info (* trace *)
+                        * excOn Y A. (* error monad *)
+
+  (* max steps handling is not totally accurate as we cannot pass the current number of steps into the function in bind, but anyways *)
+  Instance trace_monad : Monad TraceM := 
+    {| 
+      ret := fun T t => (0, [], ret t);
+      bind := fun T U x f => 
+        match x with 
+        | (s, t, e) => 
+            match e with 
+            | inl e => 
+                match f e with 
+                | (s', t', e') => 
+                    let s'' := 1 + s' + s in
+                    if Nat.leb max_steps s'' then (s'', t' ++ t, raise timeout) 
+                      else (s'', t' ++ t, e')
+                end
+            | inr err => (s, t, inr err)
+            end
+        end
+    |}. 
+
+  (* emit a trace element *)
+  Definition trace (i : trace_info) : TraceM unit := (0, [i], ret tt). 
+  Definition step : TraceM unit := (1, [], ret tt). 
+
+
+  (** Lifting of the primitive operations on the except monad *)
+  Notation "'trc' A" := (@TraceM A) (at level 100).
+
+  Definition raise {X} (y : Y) : trc X := (0, [], Except.raise y).  
+  Definition except {X} (y: Y) (a : option X) : trc X := (0, [], Except.except y a). 
+
+  Class TrcUnwrap (Xl : Type -> Type) := trc_unwrap X : Xl (trc X) -> trc (Xl X).
+  Arguments trc_unwrap {_ _ _}. 
+
+  Fixpoint list_unwrap {X : Type} (l : list (trc X)) : trc (list X) := 
+    match l with 
+    | [] => ret []
+    | x :: l => 
+        x <- x;;
+        l <- list_unwrap l;;
+        ret (x :: l)
+    end.
+  Instance list_trc_unwrap: TrcUnwrap list := @list_unwrap. 
+
+  Definition lift_exc {X} (a : excOn Y X) : trc X := (0, [], a).
+  Definition add_trace {Z} steps trace (a : trc Z) := 
+    match a with 
+    | (steps', trace', z) => (steps + steps', trace' ++ trace, z)
+    end.
+
+  Definition assert (b : bool) (err : Y) : trc unit := 
+    lift_exc (Except.assert b err). 
+
+  Definition catchE {X} (a : trc X) (f : Y -> trc X) : trc X := 
+    match a with 
+    | (steps, trace, e) => 
+        match e with 
+        | inl a => (steps, trace, e)
+        | inr e => 
+            add_trace steps trace (f e)
+        end
+    end.
+
+  Definition catch {X} (a : trc X) (f : Y -> X) : X := 
+    match a with 
+    | (_, _, inr e) => f e
+    | (_, _, inl e) => e
+    end.
+
+  Definition catchMap {X Z} (e : trc X) (f : Y -> trc Z) (g : X -> trc Z) : trc Z :=
+    match e with
+    | (steps, trace, inr e) => 
+        add_trace steps trace (f e)
+    | (steps, trace, inl a) => 
+        add_trace steps trace (g a)
+    end.
+End trace.
+
+Arguments trc_unwrap {_ _ _ _}. 
+
+Module example. 
+  Inductive err := 
+  | TimeoutErr
+  | OtherErr (s : string). 
+
+  Definition max_steps := 2. 
+  
+  Instance: Monad (@TraceM err) := @trace_monad max_steps err TimeoutErr. 
+  Notation "'trc' A" := (@TraceM err A) (at level 100). 
+
+  Definition test : trc unit := 
+    trace "test";; 
+    raise $ OtherErr "s".
+
+  Definition test' : trc unit := 
+    catchE test (fun _ => step;; raise $ OtherErr "sss"). 
+  (*Eval cbn in test'.*)
+End example.
