guarded/plugin.v
@@ -1,0 +1,196 @@
+From MetaCoq.Template Require Import Environment utils.MCRTree Ast AstUtils All. 
+Open Scope string_scope.
+Require Import List String.
+Import ListNotations.
+Open Scope string_scope.
+From MetaCoq.Guarded Require Import Inductives Except Trace.
+
+
+(* explicit instantiation with TemplateMonad as a definition parametric over the monad causes trouble with universe polymorphism *)
+Definition list_iter {X} (f : X -> TemplateMonad unit) (l : list X) : TemplateMonad unit := 
+  List.fold_left (fun (acc : TemplateMonad unit) x => _ <- acc;; f x) l (ret tt).
+
+
+
+(* whoops, I've turned the guardedness checker off *)
+Unset Guard Checking.
+
+
+Fixpoint check_fix_term (Σ : global_env) (Γ : context) (t : term) {struct t} := 
+  match t with 
+  | tFix mfix _ => 
+      (* TODO: we should first recursively check the body of the fix (in case of nested fixpoints!) *)
+      (*tmPrint mfix ;;*)
+      (*tmPrint Σ*)
+      (*ret tt*)
+      (*let Σ := *)
+      match (check_fix Σ Γ mfix) with
+      | (_, trace, inr e) => 
+          trace <- tmEval cbn trace;;
+          tmPrint trace;; tmPrint e
+      | _ => tmPrint "success"
+      end
+  | tCoFix mfix idx =>
+      (* TODO *)
+      ret tt
+  | tLambda na T M => 
+      _ <- check_fix_term Σ Γ T;;
+      _ <- check_fix_term Σ (Γ ,, vass na T) M;;
+      ret tt
+  | tApp u v => 
+      _ <- check_fix_term Σ Γ u;;
+      _ <- list_iter (check_fix_term Σ Γ) v;;
+      ret tt
+  | tProd na A B => 
+      _ <- check_fix_term Σ Γ A;;
+      _ <- check_fix_term Σ (Γ ,, vass na A) B;;
+      ret tt
+  | tCast C kind t => 
+      _ <- check_fix_term Σ Γ C;;
+      _ <- check_fix_term Σ Γ t;;
+      ret tt
+  | tLetIn na b t b' => 
+      _ <- check_fix_term Σ Γ b;;
+      _ <- check_fix_term Σ Γ t;;
+      _ <- check_fix_term Σ (Γ ,, vdef na b t) b';;
+      ret tt
+  | tCase ind rtf discriminant brs =>
+    _ <- check_fix_term Σ Γ rtf;;
+    _ <- check_fix_term Σ Γ discriminant;;
+    _ <- list_iter (fun '(_, b) => check_fix_term Σ Γ b) brs;;
+    ret tt
+  | tProj _ C => 
+      _ <- check_fix_term Σ Γ C;;
+      ret tt
+  | tConst kn u => 
+      match lookup_env_const Σ kn with 
+      | Some const => 
+          match const.(cst_body) with 
+          | Some t => check_fix_term Σ Γ t
+          | _ => ret tt
+          end
+      | None => ret tt
+      end
+  | _ => ret tt 
+  end.
+
+Set Guard Checking. 
+
+Definition check_fix {A} (a : A) :=
+  mlet (Σ, t) <- tmQuoteRec a ;;
+  (*tmPrint Σ;;*)
+  check_fix_term Σ [] t.
+
+
+
+(** * Some tests *)
+Unset Guard Checking.
+
+Require Import List String.
+Import MonadNotation.
+Import ListNotations.
+Open Scope string_scope.
+
+Fixpoint broken_app {A : Type} (l m : list A) {struct l} := 
+  match l with
+  | [] => m
+  | a :: l' => broken_app l m
+  end.
+
+(*Set Printing All. *)
+MetaCoq Run (check_fix broken_app ). 
+MetaCoq Run (check_fix app ). 
+MetaCoq Run (check_fix rev).
+MetaCoq Run (check_fix Nat.div).
+
+
+
+(** Rosetrees *)
+Inductive rtree (X : Type) := 
+  | rnode (children : list (rtree X)). 
+
+Fixpoint sumn (l : list nat) := List.fold_left (fun a b => a + b) l 0. 
+MetaCoq Run (check_fix sumn). 
+
+Fixpoint rtree_size {X} (t : rtree X) := 
+  match t with
+  | rnode l => sumn (map rtree_size l)
+  end.
+
+MetaCoq Run (check_fix rtree_size). 
+
+
+
+
+
+
+
+
+
+(** Vectors *)
+Set Implicit Arguments.
+Set Asymmetric Patterns.
+Require Coq.Vectors.Vector.
+
+Section ilist.
+
+(* Lists of elements whose types depend on an indexing set (CPDT's hlists).
+These lists are a convenient way to implement finite maps
+whose elements depend on their keys. The data structures used
+by our ADT notations uses these to implement notation-friendly
+method lookups. *)
+
+Import Coq.Vectors.VectorDef.VectorNotations.
+
+Context {A : Type}. (* The indexing type. *)
+Context {B : A -> Type}. (* The type of indexed elements. *)
+
+Fixpoint ilist {n} (l : Vector.t A n) : Type :=
+match l with
+| [] => unit
+| a :: l => (B a) * (ilist l)
+end.
+
+MetaCoq Run (check_fix_start ilist).
+
+Definition icons (a : A) {n} {l : Vector.t A n} (b : B a) (il : ilist l) : ilist (a :: l) := pair b il.
+
+Axiom ilist_hd : forall {n} {As : Vector.t A n} (il : ilist As),
+match As return ilist As -> Type with
+| a :: As' => fun il => B a
+| [] => fun _ => unit
+end il.
+
+Axiom ilist_tl : forall {n} {As : Vector.t A n} (il : ilist As),
+match As return ilist As -> Type with
+| a :: As' => fun il => ilist As'
+| [] => fun _ => unit
+end il.
+
+Definition ith_body 
+    (ith : forall {m : nat} {As : Vector.t A m} (il : ilist As) (n : Fin.t m), B (Vector.nth As n))
+    {m : nat}
+    {As : Vector.t A m}
+    (il : ilist As)
+    (n : Fin.t m)
+  : B (Vector.nth As n)
+:= Eval cbv beta iota zeta delta [Vector.caseS] in
+  match n in Fin.t m return forall (As : Vector.t A m), ilist As -> B (Vector.nth As n) with
+  | Fin.F1 k =>
+    fun As =>
+      Vector.caseS (fun n As => ilist As -> B (Vector.nth As (@ Fin.F1 n)))
+      (fun h n t => ilist_hd) As
+  | Fin.FS k n' =>
+    fun As =>
+      Vector.caseS (fun n As => forall n', ilist As -> B (Vector.nth As (@ Fin.FS n n')))
+        (fun h n t m il => @ ith _ _ (ilist_tl il) m)
+        As n'
+  end As il.
+
+Fixpoint ith {m : nat} {As : Vector.t A m} (il : ilist As) (n : Fin.t m) {struct n} : B (Vector.nth As n) := 
+  @ ith_body (@ ith) m As il n.
+
+(* TODO: diverges *)
+(*MetaCoq Run (check_fix_start ith).*)
+
+
