guarded/printers.v
@@ -1,0 +1,151 @@
+(* Adapted from  https://github.com/NeuralCoder3/metacoq/blob/unary-param/translations/de_bruijn_print.v *)
+
+
+(*
+
+Pretty print for terms with bruijn indices
+(it might be easier to go the other way
+and print coq terms with indices)
+For a complete pretty print with names
+unquote and use Coqs Print Command
+It is useful as debugging if a term does not type
+ *)
+
+Require Import MetaCoq.Template.All.
+
+Require Import List String.
+Require Import Ascii.
+Require Import Program Arith Lia PeanoNat.
+Import ListNotations MonadNotation Nat.
+
+Definition ascii_to_string (a:ascii) : string := String a (EmptyString).
+Definition natToChar (n:nat) : ascii := ascii_of_nat(48+n).
+
+Program Fixpoint natToString (n:nat) {measure n} : string :=
+  match leb n 9 with
+    true =>
+    ascii_to_string (natToChar n)
+  | false =>
+    append (natToString (Nat.div n 10)) (ascii_to_string(natToChar(Nat.modulo n 10)))
+  end.
+Next Obligation.
+  symmetry in Heq_anonymous.
+  apply leb_complete_conv in Heq_anonymous.
+  pose proof (divmod_spec n 9 0 9).
+  destruct divmod.
+  destruct H;trivial.
+  cbn. lia.
+Qed.
+
+Infix ":s" := String (at level 73).
+Infix "+s" := append (at level 72).
+Definition linebreak := ascii_to_string(ascii_of_nat 10).
+
+Definition join (xs:list string) : string :=
+  fold_left append xs EmptyString.
+
+Require Import String.
+Open Scope string_scope.
+
+(* needed for mutual inductive types *)
+Definition getInductiveName Σ (ind:kername) (indIndex:nat) : string :=
+  match lookup_env Σ ind with 
+  | Some (InductiveDecl ind) => 
+      match nth_error ind.(ind_bodies) indIndex with 
+      | None => "[ind not found]"
+      | Some b => b.(ind_name)
+      end
+  | _ => "[ind not found]"
+  end.
+
+
+Definition getConstructName Σ (ind:kername) (indIndex:nat) (consIndex:nat) : string :=
+  match lookup_env Σ ind with 
+  | Some (InductiveDecl ind) => 
+      match nth_error ind.(ind_bodies) indIndex with 
+      | None => "[ctor not found]"
+      | Some b => match nth_error b.(ind_ctors) consIndex with
+                  | None => "[ctor not found]"
+                  | Some (s, _, _) => s
+                  end
+      end
+  | _ => "[ctor not found]"
+  end.
+
+Definition nameToString (s:name) : string :=
+  match s with
+    nAnon => "_"
+  | nNamed s => s
+  end.
+
+Definition concatString (xs:list string) : string :=
+  fold_left (fun a b => a +s b) xs "".
+
+(* Print kername.
+Print ident.
+Print tmQuoteInductive. *)
+
+Definition bruijn_print Σ := fix bruijn_print_aux (t:term) : string :=
+  match t with
+  | tRel n => ("R" :s (natToString n))
+  | tVar ident => (ident)
+  | tEvar n xs => "TODO:EVAR"
+  | tSort univ => 
+    "tSort ?"
+  | tProd n t t2 => match n.(binder_name) with
+                   | nAnon => let s1 := bruijn_print_aux t in
+                              let s2 := bruijn_print_aux t2 in
+                             ("(":s append s1 (append ") -> " s2))
+                   | nNamed s => let s1 := bruijn_print_aux t in
+                                 let s2 := bruijn_print_aux t2 in
+                                ("∀ (" +s s +s (" : "+s s1) +s "), " +s s2)
+                   end
+  | tLambda s t t2 => let s1 := bruijn_print_aux t in
+                      let s2 := bruijn_print_aux t2 in
+                    ("λ ("+s match s.(binder_name) with
+                        nAnon => "_"
+                      | nNamed s => s
+                      end
+                     +s " : "+s s1+s"). "+s s2)
+  | tLetIn name t1 t2 t3 =>
+    let s1 := bruijn_print_aux t1 in 
+    let s2 := bruijn_print_aux t2 in 
+    let s3 := bruijn_print_aux t3 in
+    ("let "+s (nameToString name.(binder_name)) +s " := "+s s1 +s " : " +s s2 +s " in "+s linebreak +s s3)
+  | tApp t1 t2 =>
+    let s1 := bruijn_print_aux t1 in
+    let s2 := List.fold_left (fun s t => let s2 := bruijn_print_aux t in (s +s s2 +s ";")) t2 "" in
+    ("((" +s s1 +s ") [" +s s2 +s "])")
+  | tConst kn ui => let (_,name) := kn in name
+  | tInd ind ui => getInductiveName Σ ind.(inductive_mind) ind.(inductive_ind)
+  | tConstruct ind n ui => getConstructName Σ ind.(inductive_mind) ind.(inductive_ind) n
+  | tCase ((ind,n), _) p c brs =>
+    let sc := bruijn_print_aux c in
+    let sp := bruijn_print_aux p in
+    let sb := fold_left (fun sa x => match x with (n,t) => let st := bruijn_print_aux t in (sa +s " | ("+s(natToString n)+s") " +s st +s linebreak) end) brs "" in 
+    (linebreak +s "match (P:" +s (natToString n) +s ") "+s sc +s " return " +s sp +s " with" +s linebreak +s
+            sb +s
+             "end")
+  | tProj p t => "TODO:Proj"
+  | tFix mf n =>
+    (fix f xs := match xs with
+                  nil => ""
+                | mfb::xs =>
+                  let sr := f xs in
+          let stype := bruijn_print_aux (mfb.(dtype)) in 
+          let sbody := bruijn_print_aux (mfb.(dbody)) in
+          (linebreak +s "(fix "+s (nameToString mfb.(dname).(binder_name)) +s " : " +s stype +s " := " +s linebreak +s sbody +s ") "+s sr)
+                end
+    ) mf
+  | _ => "TODO"
+  end.
+
+
+Definition printTest := 
+  (forall (P:nat->Prop) (H0:P 0) (HS: forall n, P n -> P (S n)) (n:nat), P n).
+
+(*Definition test : TemplateMonad unit := *)
+  (*mlet (Σ, t) <- tmQuoteRec printTest;;*)
+  (*s <- tmEval cbn (bruijn_print Σ t);;*)
+  (*tmPrint  s. *)
+(*MetaCoq Run test. *)
