guarded/util.v
@@ -1,0 +1,46 @@
+From MetaCoq.Template Require Import utils.
+Require Import MetaCoq.Guarded.Except.
+
+Definition map2_i { A B C} (f : nat -> A -> B -> C) (a : list A) (b : list B) := 
+  let map2' := fix rec a b n := 
+     match a, b with
+     | a0 :: a, b0 :: b => f n a0 b0 :: rec a b (S n)
+     | _, _ => []
+     end
+  in map2' a b 0.
+Fixpoint update_list {X} (l : list X) index x := 
+  match l with 
+  | [] => []
+  | h :: l => 
+      match index with 
+      | 0 => x :: l
+      | S index => h :: update_list l index x
+      end
+  end.
+
+Section Except. 
+  Context { Y : Type}. 
+  (*Notation "'exc' X" := (excOn Y X) (at level 100). *)
+  Context {M : Type -> Type} {M_monad : Monad M}. 
+
+  Definition list_iter {X} (f : X -> M unit) (l : list X) : M unit := 
+    List.fold_left (fun (acc : M unit) x => _ <- acc;; f x) l (ret tt).
+  Definition list_iteri {X} (f : nat -> X -> M unit) (l : list X) : M unit := 
+    _ <- List.fold_left (fun (acc : M nat) x => i <- acc;; _ <- f i x;; ret (S i)) l (ret 0);;
+    ret tt.
+
+
+End Except.
+
+Definition hd {X} (l : list X) : option X := 
+  match l with 
+  | [] => None
+  | x :: l => Some x
+  end.
+
+Definition tl {X} (l : list X) : option(list X) := 
+  match l with 
+  | [] => None
+  | x :: l => Some l
+  end.
+
