template-coq/update_plugin.sh
@@ -2,7 +2,7 @@
 
 TOCOPY="ast_denoter.ml ast_quoter.ml denoter.ml plugin_core.ml plugin_core.mli reification.ml quoter.ml run_extractable.ml run_extractable.mli tm_util.ml"
 
-# Test is gen-src is older than src
+# Test if gen-src is older than src
 if [[ "gen-src" -ot "src" || ! -f "gen-src/denoter.ml" || ! -f "gen-src/metacoq_template_plugin.cmxs" ||
   "gen-src/extractable.ml" -nt "gen-src/metacoq_template_plugin.cmxs" ]]
 then
